Added all lemmas for generic map

alpha_map/Grows-only_map/App_alpha_map.fst
@@ -12,18 +12,18 @@ let concrete_st_s = S.t nat
 let init_st_s : concrete_st_s = S.empty
 
 //operation type of gset
-type op_s : eqtype =
-  |Add : nat (*value*) -> op_s
+type app_op_s : eqtype =
+  |Add : nat (*value*) -> app_op_s
 
 let get_ele (_,(_,Add e)) = e
 
 ////do function of gset
-let do_s (s:concrete_st_s) (o:(nat & (nat & op_s))) =
+let do_s (s:concrete_st_s) (o:op_s) =
   match o with
   |(_,(_,Add e)) -> S.add e s
 
 //conflict resolution of gset
-let rc_s (o1 o2:(nat & (nat & op_s))) : rc_res = Either
+let rc_s (o1 o2:op_s) : rc_res = Either
 
 //three-way merge of gset
 let merge_s (l a b:concrete_st_s) : concrete_st_s =
@@ -66,37 +66,349 @@ let lemma_merge (l a b:concrete_st)
 
 ////////////////////////////////////////////////////////////////////////////
 
-(*Two OP COMM*)
 #set-options "--z3rlimit 100 --ifuel 3"
-let comm_ind_right_s (l a b:concrete_st_s) (o1 o2' o2:(nat & (nat & op_s)))
-  : Lemma (requires Either? (rc_s o1 o2) /\
-                    eq_s (merge_s l (do_s a o1) (do_s b o2)) (do_s (do_s (merge_s l a b) o2) o1))
+(*Two OP RC*)
+//////////////// 
+let rc_ind_right_s (l a b:concrete_st_s) (o1 o2 o2':op_s)
+  : Lemma (requires rc_s o1 o2 <> Either /\ distinct_ops o1 o2 /\ distinct_ops o1 o2' /\ distinct_ops o2 o2' /\ 
+                    eq_s (merge_s l (do_s a o1) (do_s b o2)) (do_s (merge_s l (do_s a o1) b) o2))
+          (ensures eq_s (merge_s l (do_s a o1) (do_s (do_s b o2') o2)) (do_s (merge_s l (do_s a o1) (do_s b o2')) o2)) = ()
+
+let rc_ind_right_ne (l a b:concrete_st) (o1 o2 o2':op_t)
+  : Lemma (requires Fst_then_snd? (rc o1 o2) /\
+                    distinct_ops o1 o2 /\ distinct_ops o1 o2' /\ distinct_ops o2 o2' /\  
+                    ~ (get_key o1 = get_key o2 /\ get_key o2 = get_key o2') /\
+                    eq (merge l (do a o1) (do b o2)) (do (merge l (do a o1) b) o2))
+          (ensures eq (merge l (do a o1) (do (do b o2') o2)) (do (merge l (do a o1) (do b o2')) o2)) = ()
+          
+let rc_ind_left_s (l a b:concrete_st_s) (o1 o2 o1':op_s)
+  : Lemma (requires rc_s o1 o2 <> Either /\ distinct_ops o1 o2 /\ distinct_ops o1 o1' /\ distinct_ops o2 o1' /\  
+                    eq_s (merge_s l (do_s a o1) (do_s b o2)) (do_s (merge_s l (do_s a o1) b) o2))
+          (ensures eq_s (merge_s l (do_s (do_s a o1') o1) (do_s b o2)) (do_s (merge_s l (do_s (do_s a o1') o1) b) o2)) = ()
+
+let rc_ind_left_ne (l a b:concrete_st) (o1 o2 o1':op_t)
+  : Lemma (requires Fst_then_snd? (rc o1 o2) /\
+                    distinct_ops o1 o2 /\ distinct_ops o1 o1' /\ distinct_ops o2 o1' /\  
+                    ~ (get_key o1 = get_key o2 /\ get_key o2 = get_key o1') /\
+                    eq (merge l (do a o1) (do b o2)) (do (merge l (do a o1) b) o2))
+          (ensures eq (merge l (do (do a o1') o1) (do b o2)) (do (merge l (do (do a o1') o1) b) o2)) = ()
+
+let rc_ind_lca_s (l:concrete_st_s) (o1 o2 o:op_s)
+  : Lemma (requires rc_s o1 o2 <> Either /\ distinct_ops o1 o2 /\ distinct_ops o o1 /\ distinct_ops o o2 /\
+                    eq_s (merge_s l (do_s l o1) (do_s l o2)) (do_s (do_s l o1) o2))
+          (ensures eq_s (merge_s (do_s l o) (do_s (do_s l o) o1) (do_s (do_s l o) o2)) (do_s (do_s (do_s l o) o1) o2)) = ()
+
+let rc_ind_lca_ne (l:concrete_st) (o1 o2 o:op_t)
+  : Lemma (requires Fst_then_snd? (rc o1 o2) /\ 
+                    distinct_ops o1 o2 /\ distinct_ops o1 o /\ distinct_ops o o2 /\
+                    ~ (get_key o1 = get_key o2 /\ get_key o2 = get_key o) /\
+                    eq (merge l (do l o1) (do l o2)) (do (do l o1) o2))
+          (ensures eq (merge (do l o) (do (do l o) o1) (do (do l o) o2)) (do (do (do l o) o1) o2)) = ()
+
+let rc_base (o1 o2:op_t)
+  : Lemma (requires Fst_then_snd? (rc o1 o2) /\ distinct_ops o1 o2)
+          (ensures eq (merge init_st (do init_st o1) (do init_st o2)) (do (do init_st o1) o2)) = ()
+          
+let rc_inter_base_right_s (l a b c:concrete_st_s) (o1 o2 ob ol:op_s)
+  : Lemma (requires rc_s o1 o2 <> Either /\ rc_s ob ol <> Either /\ 
+                    distinct_ops o1 o2 /\ distinct_ops o1 ob /\ distinct_ops o1 ol /\ distinct_ops o2 ob /\ distinct_ops o2 ol /\ distinct_ops ob ol /\ 
+                    eq_s (merge_s (do_s l ol) (do_s (do_s a ol) o1) (do_s (do_s b ol) o2)) (do_s (do_s (do_s c ol) o1) o2) /\
+                    eq_s (merge_s l (do_s a o1) (do_s b o2)) (do_s (do_s c o1) o2) /\
+                    eq_s (merge_s l (do_s a ol) (do_s b ob)) (do_s (do_s c ob) ol)) //***EXTRA***
+          (ensures eq_s (merge_s (do_s l ol) (do_s (do_s a ol) o1) (do_s (do_s (do_s b ob) ol) o2)) (do_s (do_s (do_s (do_s c ob) ol) o1) o2)) = ()
+
+let rc_inter_base_right_ne (l a b c:concrete_st) (o1 o2 ob ol:op_t) 
+  : Lemma (requires Fst_then_snd? (rc o1 o2) /\ Fst_then_snd? (rc ob ol) /\ 
+                    distinct_ops o1 o2 /\ distinct_ops o1 ob /\ distinct_ops o1 ol /\ distinct_ops o2 ob /\ distinct_ops o2 ol /\ distinct_ops ob ol /\ 
+                    ~ (get_key o1 = get_key o2 /\ get_key o2 = get_key ob) /\
+                    eq (merge (do l ol) (do (do a ol) o1) (do (do b ol) o2)) (do (do (do c ol) o1) o2) /\
+                    eq (merge l (do a o1) (do b o2)) (do (do c o1) o2) /\
+                    eq (merge l (do a ol) (do b ob)) (do (do c ob) ol)) //***EXTRA***
+          (ensures eq (merge (do l ol) (do (do a ol) o1) (do (do (do b ob) ol) o2)) (do (do (do (do c ob) ol) o1) o2)) = ()
+          
+let rc_inter_base_left_s (l a b c:concrete_st_s) (o1 o2 ob ol:op_s)
+  : Lemma (requires rc_s o1 o2 <> Either /\ rc_s ob ol <> Either /\ 
+                    distinct_ops o1 o2 /\ distinct_ops o1 ob /\ distinct_ops o1 ol /\ distinct_ops o2 ob /\ distinct_ops o2 ol /\ distinct_ops ob ol /\ 
+                    eq_s (merge_s (do_s l ol) (do_s (do_s a ol) o1) (do_s (do_s b ol) o2)) (do_s (do_s (do_s c ol) o1) o2) /\
+                    eq_s (merge_s l (do_s a o1) (do_s b o2)) (do_s (do_s c o1) o2) /\
+                    eq_s (merge_s l (do_s a ob) (do_s b ol)) (do_s (do_s c ob) ol)) //***EXTRA***
+          (ensures eq_s (merge_s (do_s l ol) (do_s (do_s (do_s a ob) ol) o1) (do_s (do_s b ol) o2)) (do_s (do_s (do_s (do_s c ob) ol) o1) o2)) = ()
+
+let rc_inter_base_left_ne (l a b c:concrete_st) (o1 o2 ob ol:op_t) 
+  : Lemma (requires Fst_then_snd? (rc o1 o2) /\ Fst_then_snd? (rc ob ol) /\ 
+                    distinct_ops o1 o2 /\ distinct_ops o1 ob /\ distinct_ops o1 ol /\ distinct_ops o2 ob /\ distinct_ops o2 ol /\ distinct_ops ob ol /\ 
+                    ~ (get_key o1 = get_key o2 /\ get_key o2 = get_key ob) /\
+                    eq (merge (do l ol) (do (do a ol) o1) (do (do b ol) o2)) (do (do (do c ol) o1) o2) /\
+                    eq (merge l (do a o1) (do b o2)) (do (do c o1) o2) /\
+                    eq (merge l (do a ob) (do b ol)) (do (do c ob) ol)) //***EXTRA***
+          (ensures eq (merge (do l ol) (do (do (do a ob) ol) o1) (do (do b ol) o2)) (do (do (do (do c ob) ol) o1) o2)) = ()
+          
+let rc_inter_right_s (l a b c:concrete_st_s) (o1 o2 ob ol o:op_s)
+  : Lemma (requires rc_s o1 o2 <> Either /\ rc_s ob ol <> Either /\ 
+                    distinct_ops o1 o2 /\ distinct_ops o1 ob /\ distinct_ops o1 ol /\ distinct_ops o1 o /\ distinct_ops o2 ob /\ 
+                    distinct_ops o2 ol /\ distinct_ops o2 o /\ distinct_ops ob ol /\ distinct_ops ob o /\ distinct_ops ol o /\
+                    get_rid o <> get_rid ol /\
+
+                    eq_s (merge_s (do_s l ol) (do_s (do_s a ol) o1) (do_s (do_s (do_s b ob) ol) o2)) (do_s (do_s (do_s (do_s c ob) ol) o1) o2))
+      (ensures eq_s (merge_s (do_s l ol) (do_s (do_s a ol) o1) (do_s (do_s (do_s (do_s b o) ob) ol) o2)) (do_s (do_s (do_s (do_s (do_s c o) ob) ol) o1) o2)) = ()
+
+let rc_inter_right_ne (l a b c:concrete_st) (o1 o2 ob ol o:op_t) 
+  : Lemma (requires Fst_then_snd? (rc o1 o2) /\ Fst_then_snd? (rc ob ol) /\ 
+                    distinct_ops o1 o2 /\ distinct_ops o1 ob /\ distinct_ops o1 ol /\ distinct_ops o1 o /\ distinct_ops o2 ob /\ 
+                    distinct_ops o2 ol /\ distinct_ops o2 o /\ distinct_ops ob ol /\ distinct_ops ob o /\ distinct_ops ol o /\
+                    ~ (get_key o1 = get_key o2 /\ get_key o2 = get_key ob) /\
+                    get_rid o <> get_rid ol (*o,ol must be concurrent*) /\
+                    ((~ (commutes_with o ob)) \/ Fst_then_snd? (rc o ol)) /\
+                    eq (merge (do l ol) (do (do a ol) o1) (do (do (do b ob) ol) o2)) (do (do (do (do c ob) ol) o1) o2))
+      (ensures eq (merge (do l ol) (do (do a ol) o1) (do (do (do (do b o) ob) ol) o2)) (do (do (do (do (do c o) ob) ol) o1) o2)) = ()
+      
+let rc_inter_left_s (l a b c:concrete_st_s) (o1 o2 ob ol o:op_s)
+  : Lemma (requires rc_s o1 o2 <> Either /\ rc_s ob ol <> Either /\ 
+                    distinct_ops o1 o2 /\ distinct_ops o1 ob /\ distinct_ops o1 ol /\ distinct_ops o1 o /\ distinct_ops o2 ob /\ 
+                    distinct_ops o2 ol /\ distinct_ops o2 o /\ distinct_ops ob ol /\ distinct_ops ob o /\ distinct_ops ol o /\
+                    get_rid o <> get_rid ol /\
+
+                    eq_s (merge_s (do_s l ol) (do_s (do_s (do_s a ob) ol) o1) (do_s (do_s b ol) o2)) (do_s (do_s (do_s (do_s c ob) ol) o1) o2))
+      (ensures eq_s (merge_s (do_s l ol) (do_s (do_s (do_s (do_s a o) ob) ol) o1) (do_s (do_s b ol) o2)) (do_s (do_s (do_s (do_s (do_s c o) ob) ol) o1) o2)) = ()
+
+let rc_inter_left_ne (l a b c:concrete_st) (o1 o2 ob ol o:op_t) 
+  : Lemma (requires Fst_then_snd? (rc o1 o2) /\ Fst_then_snd? (rc ob ol) /\ 
+                    distinct_ops o1 o2 /\ distinct_ops o1 ob /\ distinct_ops o1 ol /\ distinct_ops o1 o /\ distinct_ops o2 ob /\ 
+                    distinct_ops o2 ol /\ distinct_ops o2 o /\ distinct_ops ob ol /\ distinct_ops ob o /\ distinct_ops ol o /\
+                    ~ (get_key o1 = get_key o2 /\ get_key o2 = get_key ob) /\
+                    get_rid o <> get_rid ol (*o,ol must be concurrent*) /\
+                    ((~ (commutes_with o ob)) \/ Fst_then_snd? (rc o ol)) /\
+                    eq (merge (do l ol) (do (do (do a ob) ol) o1) (do (do b ol) o2)) (do (do (do (do c ob) ol) o1) o2))
+      (ensures eq (merge (do l ol) (do (do (do (do a o) ob) ol) o1) (do (do b ol) o2)) (do (do (do (do (do c o) ob) ol) o1) o2)) = ()
+
+// In general, the events ol,oi, below should be such that these exists o, (rc o ol), (rc o oi)
+let rc_inter_lca_s (l a b c:concrete_st_s) (o1 o2 ol oi:op_s)
+  : Lemma (requires rc_s o1 o2 <> Either /\ 
+                    distinct_ops o1 o2 /\ distinct_ops o1 ol /\ distinct_ops o1 oi /\ distinct_ops o2 ol /\ distinct_ops o2 oi /\ distinct_ops ol oi /\
+                    (exists o. rc_s o ol <> Either) /\ 
+                    (exists o. rc_s o oi <> Either) /\
+                    eq_s (merge_s (do_s l oi) (do_s (do_s a oi) o1) (do_s (do_s b oi) o2)) (do_s (do_s (do_s c oi) o1) o2) /\
+                    eq_s (merge_s (do_s l ol) (do_s (do_s a ol) o1) (do_s (do_s b ol) o2)) (do_s (do_s (do_s c ol) o1) o2))
+    (ensures eq_s (merge_s (do_s (do_s l oi) ol) (do_s (do_s (do_s a oi) ol) o1) (do_s (do_s (do_s b oi) ol) o2)) (do_s (do_s (do_s (do_s c oi) ol) o1) o2)) = ()
+
+let rc_inter_lca_ne (l a b c:concrete_st) (o1 o2 ol oi:op_t) 
+  : Lemma (requires Fst_then_snd? (rc o1 o2) /\ 
+                    distinct_ops o1 o2 /\ distinct_ops o1 ol /\ distinct_ops o1 oi /\ distinct_ops o2 ol /\ distinct_ops o2 oi /\ distinct_ops ol oi /\
+                    ~ (get_key o1 = get_key o2 /\ get_key o1 = get_key oi /\ get_key o1 = get_key ol) /\
+                    
+                    (exists o. Fst_then_snd? (rc o ol)) /\ 
+                    (exists o. Fst_then_snd? (rc o oi)) /\ 
+                    eq (merge (do l oi) (do (do a oi) o1) (do (do b oi) o2)) (do (do (do c oi) o1) o2) /\
+                    eq (merge (do l ol) (do (do a ol) o1) (do (do b ol) o2)) (do (do (do c ol) o1) o2))
+    (ensures eq (merge (do (do l oi) ol) (do (do (do a oi) ol) o1) (do (do (do b oi) ol) o2)) (do (do (do (do c oi) ol) o1) o2)) = ()
+
+(*One op*)
+///////////////
+let one_op_ind_right_s (l a b:concrete_st_s) (o2 o2':op_s) 
+  : Lemma (requires distinct_ops o2 o2' /\ 
+                    eq_s (merge_s l a (do_s b o2)) (do_s (merge_s l a b) o2))
+           (ensures eq_s (merge_s l a (do_s (do_s b o2') o2)) (do_s (merge_s l a (do_s b o2')) o2)) = ()
+
+let one_op_ind_right_ne (l a b:concrete_st) (o2 o2':op_t)
+  : Lemma (requires distinct_ops o2 o2' /\ 
+                    ~ (get_key o2 = get_key o2') /\
+                    eq (merge l a (do b o2)) (do (merge l a b) o2))
+           (ensures eq (merge l a (do (do b o2') o2)) (do (merge l a (do b o2')) o2)) = ()
+
+let one_op_ind_left_s (l a b:concrete_st_s) (o1 o1':op_s) 
+  : Lemma (requires distinct_ops o1 o1' /\ 
+                    eq_s (merge_s l (do_s a o1) b) (do_s (merge_s l a b) o1))
+           (ensures eq_s (merge_s l (do_s (do_s a o1') o1) b) (do_s (merge_s l (do_s a o1') b) o1)) = ()
+
+let one_op_ind_left_ne (l a b:concrete_st) (o1 o1':op_t)
+   : Lemma (requires distinct_ops o1 o1' /\ 
+                     ~ (get_key o1 = get_key o1') /\
+                    eq (merge l (do a o1) b) (do (merge l a b) o1))
+           (ensures eq (merge l (do (do a o1') o1) b) (do (merge l (do a o1') b) o1)) = ()
+           
+let one_op_ind_lca_s (l:concrete_st_s) (o2 o:op_s) 
+  : Lemma (requires distinct_ops o2 o /\ 
+                    eq_s (merge_s l l (do_s l o2)) (do_s l o2))
+          (ensures eq_s (merge_s (do_s l o) (do_s l o) (do_s (do_s l o) o2)) (do_s (do_s l o) o2)) = () 
+
+let one_op_ind_lca_ne (l:concrete_st) (o2 o:op_t)
+   : Lemma (requires distinct_ops o2 o /\ 
+                     ~ (get_key o2 = get_key o) /\
+                     eq (merge l l (do l o2)) (do l o2))
+          (ensures eq (merge (do l o) (do l o) (do (do l o) o2)) (do (do l o) o2)) = ()
+
+let one_op_base (o2:op_t)
+  : Lemma (ensures eq (merge init_st init_st (do init_st o2)) (do init_st o2)) = ()
+
+let one_op_inter_base_right_s (l a b c:concrete_st_s) (o2 ob ol:op_s)
+  : Lemma (requires rc_s ob ol <> Either /\ 
+                    distinct_ops o2 ob /\ distinct_ops o2 ol /\ distinct_ops ob ol /\ 
+                    eq_s (merge_s (do_s l ol) (do_s a ol) (do_s (do_s b ol) o2)) (do_s (do_s c ol) o2) /\
+                    eq_s (merge_s l a (do_s b o2)) (do_s c o2) /\
+                    eq_s (merge_s l (do_s a ol) (do_s b ob)) (do_s (do_s c ob) ol)) //***EXTRA***
+          (ensures eq_s (merge_s (do_s l ol) (do_s a ol) (do_s (do_s (do_s b ob) ol) o2)) (do_s (do_s (do_s c ob) ol) o2)) = ()
+
+let one_op_inter_base_right_ne (l a b c:concrete_st) (o2 ob ol:op_t) 
+  : Lemma (requires Fst_then_snd? (rc ob ol) /\ 
+                    distinct_ops o2 ob /\ distinct_ops o2 ol /\ distinct_ops ob ol /\ 
+                    ~ (get_key o2 = get_key ob) /\
+                    eq (merge (do l ol) (do a ol) (do (do b ol) o2)) (do (do c ol) o2) /\
+                    eq (merge l a (do b o2)) (do c o2) /\
+                    eq (merge l (do a ol) (do b ob)) (do (do c ob) ol)) //***EXTRA***
+          (ensures eq (merge (do l ol) (do a ol) (do (do (do b ob) ol) o2)) (do (do (do c ob) ol) o2)) = ()
+
+let one_op_inter_base_left_s (l a b c:concrete_st_s) (o2 ob ol:op_s)
+  : Lemma (requires rc_s ob ol <> Either /\ 
+                    distinct_ops o2 ob /\ distinct_ops o2 ol /\ distinct_ops ob ol /\ 
+                    eq_s (merge_s (do_s l ol) (do_s a ol) (do_s (do_s b ol) o2)) (do_s (do_s c ol) o2) /\
+                    eq_s (merge_s l a (do_s b o2)) (do_s c o2) /\
+                    eq_s (merge_s l (do_s a ol) (do_s b ob)) (do_s (do_s c ob) ol) /\ //***EXTRA***
+                    eq_s (merge_s l (do_s (do_s a ob) ol) (do_s b ol)) (do_s (do_s c ob) ol)) //***EXTRA***
+          (ensures eq_s (merge_s (do_s l ol) (do_s (do_s a ob) ol) (do_s (do_s b ol) o2)) (do_s (do_s (do_s c ob) ol) o2)) = ()
+
+let one_op_inter_base_left_ne (l a b c:concrete_st) (o2 ob ol:op_t) 
+  : Lemma (requires Fst_then_snd? (rc ob ol) /\
+                    distinct_ops o2 ob /\ distinct_ops o2 ol /\ distinct_ops ob ol /\
+                    ~ (get_key o2 = get_key ob) /\
+                    eq (merge (do l ol) (do a ol) (do (do b ol) o2)) (do (do c ol) o2) /\
+                    (Fst_then_snd? (rc ob o2) ==> eq (merge l (do a o2) (do b ob)) (do (merge l a (do b ob)) o2)) /\ //***EXTRA***
+                    eq (merge l a (do b o2)) (do c o2) /\
+                    eq (merge l (do a ol) (do b ob)) (do (do c ob) ol) /\ //***EXTRA***
+                    eq (merge l (do (do a ob) ol) (do b ol)) (do (do c ob) ol)) //***EXTRA***
+          (ensures eq (merge (do l ol) (do (do a ob) ol) (do (do b ol) o2)) (do (do (do c ob) ol) o2)) = ()
+          
+let one_op_inter_right_s (l a b c:concrete_st_s) (o2 ob ol o:op_s)
+  : Lemma (requires rc_s ob ol <> Either /\ 
+                    distinct_ops o ob /\ distinct_ops o ol /\ distinct_ops o o2 /\ distinct_ops ob ol /\ distinct_ops ob o2 /\ distinct_ops o2 ol /\
+                    get_rid o <> get_rid ol /\
+                    eq_s (merge_s (do_s l ol) (do_s a ol) (do_s (do_s (do_s b ob) ol) o2)) (do_s (do_s (do_s c ob) ol) o2))
+      (ensures eq_s (merge_s (do_s l ol) (do_s a ol) (do_s (do_s (do_s (do_s b o) ob) ol) o2)) (do_s (do_s (do_s (do_s c o) ob) ol) o2)) = ()
+
+let one_op_inter_right_ne (l a b c:concrete_st) (o2 ob ol o:op_t) 
+  : Lemma (requires Fst_then_snd? (rc ob ol) /\
+                    distinct_ops o ob /\ distinct_ops o ol /\ distinct_ops o o2 /\ distinct_ops ob ol /\ distinct_ops ob o2 /\ distinct_ops o2 ol /\
+                    get_rid o <> get_rid ol (*o,ol must be concurrent*) /\
+                    ((~ (commutes_with o ob)) \/ Fst_then_snd? (rc o ol)) /\
+                    eq (merge (do l ol) (do a ol) (do (do (do b ob) ol) o2)) (do (do (do c ob) ol) o2))
+          (ensures eq (merge (do l ol) (do a ol) (do (do (do (do b o) ob) ol) o2)) (do (do (do (do c o) ob) ol) o2)) = ()
+          
+let one_op_inter_left_s (l a b c:concrete_st_s) (o2 ob ol o:op_s)
+  : Lemma (requires rc_s ob ol <> Either /\ 
+                    distinct_ops o ob /\ distinct_ops o ol /\ distinct_ops o o2 /\ distinct_ops ob ol /\ distinct_ops ob o2 /\ distinct_ops o2 ol /\
+                    get_rid o <> get_rid ol /\
+                    eq_s (merge_s (do_s l ol) (do_s (do_s a ob) ol) (do_s (do_s b ol) o2)) (do_s (do_s (do_s c ob) ol) o2))
+          (ensures eq_s (merge_s (do_s l ol) (do_s (do_s (do_s a o) ob) ol) (do_s (do_s b ol) o2)) (do_s (do_s (do_s (do_s c o) ob) ol) o2)) = ()
+
+let one_op_inter_left_ne (l a b c:concrete_st) (o2 ob ol o:op_t) 
+  : Lemma (requires Fst_then_snd? (rc ob ol) /\
+                    distinct_ops o ob /\ distinct_ops o ol /\ distinct_ops o ol /\ distinct_ops ob ol /\ distinct_ops ob o2 /\ distinct_ops o2 ol /\
+                    ~ (get_key o2 = get_key ob) /\
+                    get_rid o <> get_rid ol (*o,ol must be concurrent*) /\
+                    ((~ (commutes_with o ob)) \/ Fst_then_snd? (rc o ol)) /\
+                    eq (merge (do l ol) (do (do a ob) ol) (do (do b ol) o2)) (do (do (do c ob) ol) o2))
+          (ensures eq (merge (do l ol) (do (do (do a o) ob) ol) (do (do b ol) o2)) (do (do (do (do c o) ob) ol) o2)) = ()
+
+// In general, the events o',o_n, below should be such that these exists o, (rc o o')
+let one_op_inter_lca_s (l a b c:concrete_st_s) (o2 ol oi:op_s)
+  : Lemma (requires distinct_ops o2 ol /\ distinct_ops o2 oi /\ distinct_ops ol oi /\ 
+                    (exists o. rc_s o ol <> Either) /\ 
+                    (exists o. rc_s o oi <> Either) /\
+                    eq_s (merge_s (do_s l oi) (do_s a oi) (do_s (do_s b oi) o2)) (do_s (do_s c oi) o2) /\
+                    eq_s (merge_s (do_s l ol) (do_s a ol) (do_s (do_s b ol) o2)) (do_s (do_s c ol) o2))
+    (ensures eq_s (merge_s (do_s (do_s l oi) ol) (do_s (do_s a oi) ol) (do_s (do_s (do_s b oi) ol) o2)) (do_s (do_s (do_s c oi) ol) o2)) = ()
+
+let one_op_inter_lca_ne (l a b c:concrete_st) (o2 ol oi:op_t)
+  : Lemma (requires distinct_ops o2 ol /\ distinct_ops o2 oi /\ distinct_ops ol oi /\ 
+                    ~ (get_key o2 = get_key oi /\ get_key o2 = get_key ol) /\
+                    (exists o. Fst_then_snd? (rc o ol)) /\ 
+                    (exists o. Fst_then_snd? (rc o oi)) /\ 
+                    eq (merge (do l oi) (do a oi) (do (do b oi) o2)) (do (do c oi) o2) /\
+                    eq (merge (do l ol) (do a ol) (do (do b ol) o2)) (do (do c ol) o2))
+          (ensures eq (merge (do (do l oi) ol) (do (do a oi) ol) (do (do (do b oi) ol) o2)) (do (do (do c oi) ol) o2)) = ()
+
+(*Zero op *)
+///////////////
+// because we proved that e_i^l rcp eb is not possible.
+//e_i^l vis eb is not possible
+// so either eb rcp e_i^l or eb rct e_i^l is possible
+let zero_op_inter_base_right_s (l a b c:concrete_st_s) (ob ol:op_s)
+  : Lemma (requires rc_s ob ol <> Either /\ distinct_ops ob ol /\ 
+                    eq_s (merge_s (do_s l ol) (do_s a ol) (do_s b ol)) (do_s c ol) /\
+                    eq_s (merge_s l a b) c /\
+                    eq_s (merge_s l (do_s a ol) (do_s b ob)) (do_s (do_s c ob) ol)) //***EXTRA***
+          (ensures eq_s (merge_s (do_s l ol) (do_s a ol) (do_s (do_s b ob) ol)) (do_s (do_s c ob) ol)) = () 
+
+let zero_op_inter_base_left_s (l a b c:concrete_st_s) (ob ol:op_s)
+  : Lemma (requires rc_s ob ol <> Either /\ distinct_ops ob ol /\ 
+                    eq_s (merge_s (do_s l ol) (do_s a ol) (do_s b ol)) (do_s c ol) /\
+                    eq_s (merge_s l a b) c /\
+                    eq_s (merge_s l (do_s a ob) (do_s b ol)) (do_s (do_s c ob) ol)) //***EXTRA***
+          (ensures eq_s (merge_s (do_s l ol) (do_s (do_s a ob) ol) (do_s b ol)) (do_s (do_s c ob) ol)) = () 
+
+let zero_op_inter_right_s (l a b c:concrete_st_s) (ob ol o:op_s)
+  : Lemma (requires rc_s ob ol <> Either /\ distinct_ops ob ol /\ distinct_ops ob o /\ distinct_ops ol o /\
+                    get_rid o <> get_rid ol (*o,ol must be concurrent*) /\
+                    eq_s (merge_s (do_s l ol) (do_s a ol) (do_s (do_s b ob) ol)) (do_s (do_s c ob) ol))
+          (ensures eq_s (merge_s (do_s l ol) (do_s a ol) (do_s (do_s (do_s b o) ob) ol)) (do_s (do_s (do_s c o) ob) ol)) = ()
+
+let zero_op_inter_left_s (l a b c:concrete_st_s) (ob ol o:op_s)
+  : Lemma (requires rc_s ob ol <> Either /\ distinct_ops ob ol /\ distinct_ops ob o /\ distinct_ops ol o /\
+                    get_rid o <> get_rid ol (*o,ol must be concurrent*) /\
+                    eq_s (merge_s (do_s l ol) (do_s (do_s a ob) ol) (do_s b ol)) (do_s (do_s c ob) ol))
+          (ensures eq_s (merge_s (do_s l ol) (do_s (do_s (do_s a o) ob) ol) (do_s b ol)) (do_s (do_s (do_s c o) ob) ol)) = ()
+
+// In general, the event "o" below should be such that these exists o', (rc o' o)
+let zero_op_inter_lca_v1_s (l a b c:concrete_st_s) (ol:op_s)
+  : Lemma (requires (exists o'. rc_s o' ol <> Either) /\ eq_s (merge_s l a b) c)
+          (ensures eq_s (merge_s (do_s l ol) (do_s a ol) (do_s b ol)) (do_s c ol)) = ()
+
+// In general, the events o',o_n, below should be such that these exists o, (rc o o')
+let zero_op_inter_lca_v2_s (l a b c:concrete_st_s) (ol oi:op_s)
+  : Lemma (requires distinct_ops ol oi /\
+                    (exists o. rc_s o ol <> Either) /\ 
+                    (exists o. rc_s o oi <> Either) /\ 
+                    eq_s (merge_s (do_s l oi) (do_s a oi) (do_s b oi)) (do_s c oi)  /\
+                    eq_s (merge_s (do_s l ol) (do_s a ol) (do_s b ol)) (do_s c ol))
+          (ensures eq_s (merge_s (do_s (do_s l oi) ol) (do_s (do_s a oi) ol) (do_s (do_s b oi) ol)) (do_s (do_s c oi) ol)) = ()
+
+let zero_op_inter_lca_v2_ne (l a b c:concrete_st) (ol oi:op_t)
+  : Lemma (requires distinct_ops ol oi /\
+                    ~ (get_key ol = get_key oi) /\
+                    (exists o. Fst_then_snd? (rc o ol)) /\ 
+                    (exists o. Fst_then_snd? (rc o oi)) /\
+                    eq (merge (do l oi) (do a oi) (do b oi)) (do c oi)  /\
+                    eq (merge (do l ol) (do a ol) (do b ol)) (do c ol))
+          (ensures eq (merge (do (do l oi) ol) (do (do a oi) ol) (do (do b oi) ol)) (do (do c oi) ol)) = ()
+          
+(* 2 op Comm  *)
+///////////////////
+#set-options "--z3rlimit 100 --ifuel 3" 
+let comm_ind_right_s (l a b:concrete_st_s) (o1 o2' o2:op_s)
+  : Lemma (requires eq_s (merge_s l (do_s a o1) (do_s b o2)) (do_s (do_s (merge_s l a b) o2) o1))
           (ensures eq_s (merge_s l (do_s a o1) (do_s (do_s b o2') o2)) (do_s (do_s (merge_s l a (do_s b o2')) o2) o1)) = ()
 
 let comm_ind_right_ne (l a b:concrete_st) (o1 o2' o2:op_t)
-  : Lemma (requires Either? (rc o1 o2) /\ Either? (rc_s (get_op_s o1) (get_op_s o2)) /\
+  : Lemma (requires Either? (rc o1 o2) /\
                      ~ (get_key o1 = get_key o2 /\ get_key o2 = get_key o2') /\
                     eq (merge l (do a o1) (do b o2)) (do (do (merge l a b) o2) o1))                    
           (ensures eq (merge l (do a o1) (do (do b o2') o2)) (do (do (merge l a (do b o2')) o2) o1)) = ()
 
-let comm_ind_left_s (l a b:concrete_st_s) (o1 o2' o2:(nat & (nat & op_s)))
-  : Lemma (requires Either? (rc_s o1 o2) /\
-                    eq_s (merge_s l (do_s a o1) (do_s b o2)) (do_s (do_s (merge_s l a b) o2) o1))
+let comm_ind_left_s (l a b:concrete_st_s) (o1 o2' o2:op_s)
+  : Lemma (requires eq_s (merge_s l (do_s a o1) (do_s b o2)) (do_s (do_s (merge_s l a b) o2) o1))
           (ensures eq_s (merge_s l (do_s (do_s a o2') o1) (do_s b o2)) (do_s (do_s (merge_s l (do_s a o2') b) o2) o1)) = ()
 
 let comm_ind_left_ne (l a b:concrete_st) (o1 o2' o2:op_t)
-  : Lemma (requires Either? (rc o1 o2) /\ Either? (rc_s (get_op_s o1) (get_op_s o2)) /\
+  : Lemma (requires Either? (rc o1 o2) /\
                     ~ (get_key o1 = get_key o2 /\ get_key o2 = get_key o2') /\
                     eq (merge l (do a o1) (do b o2)) (do (do (merge l a b) o2) o1))                    
           (ensures eq (merge l (do (do a o2') o1) (do b o2)) (do (do (merge l (do a o2') b) o2) o1)) = ()
 
-let comm_ind_lca_s (l:concrete_st_s) (ol o1 o2:(nat & (nat & op_s)))
-  : Lemma (requires Either? (rc_s o1 o2) /\
-                    eq_s (merge_s l (do_s l o1) (do_s l o2)) (do_s (do_s l o2) o1))
+let comm_ind_lca_s (l:concrete_st_s) (ol o1 o2:op_s)
+  : Lemma (requires eq_s (merge_s l (do_s l o1) (do_s l o2)) (do_s (do_s l o2) o1))
           (ensures eq_s (merge_s (do_s l ol) (do_s (do_s l ol) o1) (do_s (do_s l ol) o2)) (do_s (do_s (do_s l ol) o2) o1)) = ()
 
 let comm_ind_lca_ne (l:concrete_st) (ol o1 o2:op_t)
-  : Lemma (requires Either? (rc o1 o2) /\ Either? (rc_s (get_op_s o1) (get_op_s o2)) /\
+  : Lemma (requires Either? (rc o1 o2) /\
                     ~ (get_key ol = get_key o1 /\ get_key ol = get_key o2) /\
                     eq (merge l (do l o1) (do l o2)) (do (do l o2) o1))
           (ensures eq (merge (do l ol) (do (do l ol) o1) (do (do l ol) o2)) (do (do (do l ol) o2) o1)) = ()
@@ -105,4 +417,92 @@ let comm_base (o1 o2:op_t)
   : Lemma (requires distinct_ops o1 o2 /\ Either? (rc o1 o2))
           (ensures eq (merge init_st (do init_st o1) (do init_st o2)) (do (do init_st o1) o2)) = ()
 
+let comm_inter_base_right_s (l a b c:concrete_st_s) (o1 o2 ob ol:op_s) 
+  : Lemma (requires rc_s ob ol <> Either /\ 
+                    distinct_ops o1 o2 /\ distinct_ops o1 ob /\ distinct_ops o1 ol /\ distinct_ops o2 ob /\ distinct_ops o2 ol /\ distinct_ops ob ol /\
+                    eq_s (merge_s (do_s l ol) (do_s (do_s a ol) o1) (do_s (do_s b ol) o2)) (do_s (do_s (do_s c ol) o1) o2) /\ 
+                    eq_s (merge_s l (do_s a o1) (do_s b o2)) (do_s (do_s c o1) o2) /\
+                    eq_s (merge_s l (do_s a o1) (do_s (do_s b ob) o2)) (do_s (do_s (merge_s l a (do_s b ob)) o1) o2) /\ //comes from comm_ind_right
+                    eq_s (merge_s (do_s l ol) (do_s a ol) (do_s (do_s b ob) ol)) (do_s (do_s c ob) ol)) //comes from intermediate_base_zero_op
+          (ensures eq_s (merge_s (do_s l ol) (do_s (do_s a ol) o1) (do_s (do_s (do_s b ob) ol) o2)) (do_s (do_s (do_s (do_s c ob) ol) o1) o2)) = ()
 
+let comm_inter_base_right_ne (l a b c:concrete_st) (o1 o2 ob ol:op_t) 
+  : Lemma (requires Fst_then_snd? (rc ob ol) /\ 
+                    distinct_ops o1 o2 /\ distinct_ops o1 ob /\ distinct_ops o1 ol /\ distinct_ops o2 ob /\ distinct_ops o2 ol /\ distinct_ops ob ol /\
+                    ~ (get_key o2 = get_key o1 /\ get_key o1 = get_key ob) /\
+                    eq (merge (do l ol) (do (do a ol) o1) (do (do b ol) o2)) (do (do (do c ol) o1) o2) /\ 
+                    eq (merge l (do a o1) (do b o2)) (do (do c o1) o2) /\
+                    eq (merge l (do a o1) (do (do b ob) o2)) (do (do (merge l a (do b ob)) o1) o2) /\ //comes from comm_ind_right
+                    eq (merge (do l ol) (do a ol) (do (do b ob) ol)) (do (do c ob) ol)) //comes from intermediate_base_zero_op
+          (ensures eq (merge (do l ol) (do (do a ol) o1) (do (do (do b ob) ol) o2)) (do (do (do (do c ob) ol) o1) o2)) = ()
+
+let comm_inter_base_left_s (l a b c:concrete_st_s) (o1 o2 ob ol:op_s) 
+  : Lemma (requires rc_s ob ol <> Either /\ 
+                    distinct_ops o1 o2 /\ distinct_ops o1 ob /\ distinct_ops o1 ol /\ distinct_ops o2 ob /\ distinct_ops o2 ol /\ distinct_ops ob ol /\
+                    eq_s (merge_s (do_s l ol) (do_s (do_s a ol) o1) (do_s (do_s b ol) o2)) (do_s (do_s (do_s c ol) o1) o2) /\ 
+                    eq_s (merge_s l (do_s a o1) (do_s b o2)) (do_s (do_s c o1) o2) /\
+                    eq_s (merge_s l (do_s (do_s a ob) o1) (do_s b o2)) (do_s (do_s (merge_s l (do_s a ob) b) o1) o2) /\ //comes from comm_ind_left
+                    eq_s (merge_s (do_s l ol) (do_s (do_s a ob) ol) (do_s b ol)) (do_s (do_s c ob) ol)) //comes from intermediate_base_zero_op
+          (ensures eq_s (merge_s (do_s l ol) (do_s (do_s (do_s a ob) ol) o1) (do_s (do_s b ol) o2)) (do_s (do_s (do_s (do_s c ob) ol) o1) o2)) = ()
+
+let comm_inter_base_left_ne (l a b c:concrete_st) (o1 o2 ob ol:op_t) 
+  : Lemma (requires Fst_then_snd? (rc ob ol) /\ 
+                    distinct_ops o1 o2 /\ distinct_ops o1 ob /\ distinct_ops o1 ol /\ distinct_ops o2 ob /\ distinct_ops o2 ol /\ distinct_ops ob ol /\
+                    ~ (get_key o2 = get_key o1 /\ get_key o1 = get_key ob) /\
+                    eq (merge (do l ol) (do (do a ol) o1) (do (do b ol) o2)) (do (do (do c ol) o1) o2) /\ 
+                    eq (merge l (do a o1) (do b o2)) (do (do c o1) o2) /\
+                    eq (merge l (do (do a ob) o1) (do b o2)) (do (do (merge l (do a ob) b) o1) o2) /\ //comes from comm_ind_left
+                    eq (merge (do l ol) (do (do a ob) ol) (do b ol)) (do (do c ob) ol)) //comes from intermediate_base_zero_op
+          (ensures eq (merge (do l ol) (do (do (do a ob) ol) o1) (do (do b ol) o2)) (do (do (do (do c ob) ol) o1) o2)) = ()
+
+let comm_inter_right_s (l a b c:concrete_st_s) (o1 o2 ob ol o:op_s)
+  : Lemma (requires rc_s ob ol <> Either /\ 
+                    distinct_ops o1 o2 /\ distinct_ops o1 ob /\ distinct_ops o1 ol /\ distinct_ops o1 o /\ distinct_ops o2 ob /\ 
+                    distinct_ops o2 ol /\ distinct_ops o2 o /\ distinct_ops ob ol /\ distinct_ops ob o /\ distinct_ops ol o /\
+                    get_rid o <> get_rid ol (*o,ol must be concurrent*) /\
+                    eq_s (merge_s (do_s l ol) (do_s (do_s a ol) o1) (do_s (do_s (do_s b ob) ol) o2)) (do_s (do_s (do_s (do_s c ob) ol) o1) o2))
+          (ensures eq_s (merge_s (do_s l ol) (do_s (do_s a ol) o1) (do_s (do_s (do_s (do_s b o) ob) ol) o2)) (do_s (do_s (do_s (do_s (do_s c o) ob) ol) o1) o2)) = ()
+          
+let comm_inter_right_ne (l a b c:concrete_st) (o1 o2 ob ol o:op_t)
+  : Lemma (requires Either? (rc o1 o2) /\ Fst_then_snd? (rc ob ol) /\ 
+                    distinct_ops o1 o2 /\ distinct_ops o1 ob /\ distinct_ops o1 ol /\ distinct_ops o1 o /\ distinct_ops o2 ob /\ 
+                    distinct_ops o2 ol /\ distinct_ops o2 o /\ distinct_ops ob ol /\ distinct_ops ob o /\ distinct_ops ol o /\
+                    ~ (get_key o1 = get_key o2 /\ get_key o2 = get_key ob) /\
+                    get_rid o <> get_rid ol (*o,ol must be concurrent*) /\
+                    //Either? (rc o ol) /\ 
+                    ((~ (commutes_with o ob)) \/ Fst_then_snd? (rc o ol)) /\
+                    eq (merge (do l ol) (do (do a ol) o1) (do (do (do b ob) ol) o2)) (do (do (do (do c ob) ol) o1) o2))
+          (ensures eq (merge (do l ol) (do (do a ol) o1) (do (do (do (do b o) ob) ol) o2)) (do (do (do (do (do c o) ob) ol) o1) o2)) = ()
+
+let comm_inter_left_s (l a b c:concrete_st_s) (o1 o2 ob ol o:op_s)
+  : Lemma (requires rc_s ob ol <> Either /\ 
+                    distinct_ops o1 o2 /\ distinct_ops o1 ob /\ distinct_ops o1 ol /\ distinct_ops o1 o /\ distinct_ops o2 ob /\ 
+                    distinct_ops o2 ol /\ distinct_ops o2 o /\ distinct_ops ob ol /\ distinct_ops ob o /\ distinct_ops ol o /\
+                    get_rid o <> get_rid ol (*o,ol must be concurrent*) /\
+                    eq_s (merge_s (do_s l ol) (do_s (do_s (do_s a ob) ol) o1) (do_s (do_s b ol) o2)) (do_s (do_s (do_s (do_s c ob) ol) o1) o2))
+          (ensures eq_s (merge_s (do_s l ol) (do_s (do_s (do_s (do_s a o) ob) ol) o1) (do_s (do_s b ol) o2)) (do_s (do_s (do_s (do_s (do_s c o) ob) ol) o1) o2)) = ()
+          
+let comm_inter_left_ne (l a b c:concrete_st) (o1 o2 ob ol o:op_t)
+  : Lemma (requires Either? (rc o1 o2) /\ Fst_then_snd? (rc ob ol) /\ 
+                    distinct_ops o1 o2 /\ distinct_ops o1 ob /\ distinct_ops o1 ol /\ distinct_ops o1 o /\ distinct_ops o2 ob /\ 
+                    distinct_ops o2 ol /\ distinct_ops o2 o /\ distinct_ops ob ol /\ distinct_ops ob o /\ distinct_ops ol o /\
+                    ~ (get_key o1 = get_key o2 /\ get_key o2 = get_key ob) /\
+                    get_rid o <> get_rid ol (*o,ol must be concurrent*) /\
+                    //Either? (rc o ol) /\ 
+                    ((~ (commutes_with o ob)) \/ Fst_then_snd? (rc o ol)) /\
+                    eq (merge (do l ol) (do (do (do a ob) ol) o1) (do (do b ol) o2)) (do (do (do (do c ob) ol) o1) o2))
+          (ensures eq (merge (do l ol) (do (do (do (do a o) ob) ol) o1) (do (do b ol) o2)) (do (do (do (do (do c o) ob) ol) o1) o2)) = ()
+
+let comm_inter_lca_s (l a b c:concrete_st_s) (o1 o2 ol:op_s)
+  : Lemma (requires distinct_ops o1 o2 /\ distinct_ops o1 ol /\ distinct_ops ol o2 /\
+                    (exists o'. rc_s o' ol <> Either) /\
+                    eq_s (merge_s l (do_s a o1) (do_s b o2)) (do_s (do_s c o1) o2))
+          (ensures eq_s (merge_s (do_s l ol) (do_s (do_s a ol) o1) (do_s (do_s b ol) o2)) (do_s (do_s (do_s c ol) o1) o2)) = ()
+
+let comm_inter_lca_ne (l a b c:concrete_st) (o1 o2 ol:op_t)
+  : Lemma (requires Either? (rc o1 o2) /\ 
+                    distinct_ops o1 o2 /\ distinct_ops o1 ol /\ distinct_ops ol o2 /\
+                    ~ ( get_key o2 = get_key o1 /\ get_key o1 = get_key ol) /\
+                    (exists o'. Fst_then_snd? (rc o' ol)) /\
+                    eq (merge l (do a o1) (do b o2)) (do (do c o1) o2))
+          (ensures eq (merge (do l ol) (do (do a ol) o1) (do (do b ol) o2)) (do (do (do c ol) o1) o2)) = ()
