interface/App_alpha_map.fsti
@@ -40,25 +40,27 @@ let eq_is_equiv (a b:concrete_st)
           (ensures eq a b) = ()
 
 //operation type of simpler MRDT
-val op_s : eqtype 
+val app_op_s : eqtype 
 
 // operation type
 type app_op_t =
-  |Set : string (*key*) -> op_s -> app_op_t 
+  |Set : string (*key*) -> app_op_s -> app_op_t 
+
+type op_s = pos (*timestamp*) & (nat (*replica ID*) & app_op_s)
 
 type op_t = pos (*timestamp*) & (nat (*replica ID*) & app_op_t)
 
 let get_rid (_,(rid,_)) = rid
 
-let distinct_ops (op1 op2:op_t) = fst op1 =!= fst op2
+let distinct_ops (ts1,_) (ts2,_) = ts1 =!= ts2
 
 type log = seq op_t
 
 //do function of simpler MRDT
-val do_s (s:concrete_st_s) (o:(nat & (nat & op_s))) : concrete_st_s
+val do_s (s:concrete_st_s) (o:op_s) : concrete_st_s
 
 //convert map operation to simpler MRDT operation
-let get_op_s (o:op_t) : (nat & (nat & op_s)) =
+let get_op_s (o:op_t) : op_s =
   match o with
   |ts, (rid, Set _ o) -> (ts,(rid,o))
 
@@ -85,10 +87,11 @@ type rc_res =
   |Either
 
 //conflict resolution of simpler MRDT
-val rc_s (o1 o2:(nat & (nat & op_s))) : rc_res
+val rc_s (o1 o2:op_s) : rc_res
 
 //conflict resolution of map
-let rc (o1 o2:op_t) : rc_res = Either
+let rc (o1 o2:op_t) : rc_res = 
+  if get_key o1 = get_key o2 then rc_s (get_op_s o1) (get_op_s o2) else Either
 
 //three-way merge of simpler MRDT
 val merge_s (l a b:concrete_st_s) : concrete_st_s
@@ -136,23 +139,598 @@ val lemma_do (s:concrete_st) (o:op_t)
 val lemma_merge (l a b:concrete_st)
   : Lemma (ensures (forall k. eq_s (sel (merge l a b) k) (merge_s (sel l k) (sel a k) (sel b k))) )
 
+(*Two OP RC*)
+//////////////// 
+val rc_ind_right_s (l a b:concrete_st_s) (o1 o2 o2':op_s) 
+  : Lemma (requires rc_s o1 o2 <> Either /\ distinct_ops o1 o2 /\ distinct_ops o1 o2' /\ distinct_ops o2 o2' /\ 
+                    eq_s (merge_s l (do_s a o1) (do_s b o2)) (do_s (merge_s l (do_s a o1) b) o2))
+          (ensures eq_s (merge_s l (do_s a o1) (do_s (do_s b o2') o2)) (do_s (merge_s l (do_s a o1) (do_s b o2')) o2))
+
+val rc_ind_right_ne (l a b:concrete_st) (o1 o2 o2':op_t)
+  : Lemma (requires Fst_then_snd? (rc o1 o2) /\
+                    distinct_ops o1 o2 /\ distinct_ops o1 o2' /\ distinct_ops o2 o2' /\  
+                    ~ (get_key o1 = get_key o2 /\ get_key o2 = get_key o2') /\
+                    eq (merge l (do a o1) (do b o2)) (do (merge l (do a o1) b) o2))
+          (ensures eq (merge l (do a o1) (do (do b o2') o2)) (do (merge l (do a o1) (do b o2')) o2))
+
+let rc_ind_right (l a b:concrete_st) (o1 o2 o2':op_t)
+  : Lemma (requires Fst_then_snd? (rc o1 o2) /\
+                    distinct_ops o1 o2 /\ distinct_ops o1 o2' /\ distinct_ops o2 o2' /\  
+                    eq (merge l (do a o1) (do b o2)) (do (merge l (do a o1) b) o2))
+          (ensures eq (merge l (do a o1) (do (do b o2') o2)) (do (merge l (do a o1) (do b o2')) o2)) =
+  assert (rc_s (get_op_s o1) (get_op_s o2) <> Either);
+  let k = get_key o2' in
+  let l' = sel l k in let a' = sel a k in let b' = sel b k in 
+  if get_key o2 = get_key o1 && get_key o1 = k then 
+    rc_ind_right_s l' a' b' (get_op_s o1) (get_op_s o2) (get_op_s o2')
+  else rc_ind_right_ne l a b o1 o2 o2'
+
+val rc_ind_left_s (l a b:concrete_st_s) (o1 o2 o1':op_s)
+  : Lemma (requires rc_s o1 o2 <> Either /\ distinct_ops o1 o2 /\ distinct_ops o1 o1' /\ distinct_ops o2 o1' /\  
+                    eq_s (merge_s l (do_s a o1) (do_s b o2)) (do_s (merge_s l (do_s a o1) b) o2))
+          (ensures eq_s (merge_s l (do_s (do_s a o1') o1) (do_s b o2)) (do_s (merge_s l (do_s (do_s a o1') o1) b) o2))
+
+val rc_ind_left_ne (l a b:concrete_st) (o1 o2 o1':op_t)
+  : Lemma (requires Fst_then_snd? (rc o1 o2) /\
+                    distinct_ops o1 o2 /\ distinct_ops o1 o1' /\ distinct_ops o2 o1' /\  
+                    ~ (get_key o1 = get_key o2 /\ get_key o2 = get_key o1') /\
+                    eq (merge l (do a o1) (do b o2)) (do (merge l (do a o1) b) o2))
+          (ensures eq (merge l (do (do a o1') o1) (do b o2)) (do (merge l (do (do a o1') o1) b) o2))
+          
+let rc_ind_left (l a b:concrete_st) (o1 o2 o1':op_t)
+  : Lemma (requires Fst_then_snd? (rc o1 o2) /\
+                    distinct_ops o1 o2 /\ distinct_ops o1 o1' /\ distinct_ops o2 o1' /\
+                    eq (merge l (do a o1) (do b o2)) (do (merge l (do a o1) b) o2))
+          (ensures eq (merge l (do (do a o1') o1) (do b o2)) (do (merge l (do (do a o1') o1) b) o2)) =
+  let k = get_key o1' in
+  let l' = sel l k in let a' = sel a k in let b' = sel b k in 
+  if get_key o2 = get_key o1 && get_key o1 = k then 
+    rc_ind_left_s l' a' b' (get_op_s o1) (get_op_s o2) (get_op_s o1')
+  else rc_ind_left_ne l a b o1 o2 o1'
+
+val rc_ind_lca_s (l:concrete_st_s) (o1 o2 o:op_s)
+  : Lemma (requires rc_s o1 o2 <> Either /\ distinct_ops o1 o2 /\ distinct_ops o o1 /\ distinct_ops o o2 /\
+                    eq_s (merge_s l (do_s l o1) (do_s l o2)) (do_s (do_s l o1) o2))
+          (ensures eq_s (merge_s (do_s l o) (do_s (do_s l o) o1) (do_s (do_s l o) o2)) (do_s (do_s (do_s l o) o1) o2))
+
+val rc_ind_lca_ne (l:concrete_st) (o1 o2 o:op_t)
+  : Lemma (requires Fst_then_snd? (rc o1 o2) /\ 
+                    distinct_ops o1 o2 /\ distinct_ops o1 o /\ distinct_ops o o2 /\
+                    ~ (get_key o1 = get_key o2 /\ get_key o2 = get_key o) /\
+                    eq (merge l (do l o1) (do l o2)) (do (do l o1) o2))
+          (ensures eq (merge (do l o) (do (do l o) o1) (do (do l o) o2)) (do (do (do l o) o1) o2))
+          
+//Special case of rc_intermediate_v1
+let rc_ind_lca (l:concrete_st) (o1 o2 o:op_t)
+  : Lemma (requires Fst_then_snd? (rc o1 o2) /\ 
+                    distinct_ops o1 o2 /\ distinct_ops o o1 /\ distinct_ops o o2 /\
+                    eq (merge l (do l o1) (do l o2)) (do (do l o1) o2))
+          (ensures eq (merge (do l o) (do (do l o) o1) (do (do l o) o2)) (do (do (do l o) o1) o2)) =
+  let k = get_key o in
+  let l' = sel l k in
+  if get_key o2 = get_key o1 && get_key o1 = k then 
+    rc_ind_lca_s l' (get_op_s o1) (get_op_s o2) (get_op_s o)
+  else rc_ind_lca_ne l o1 o2 o
+          
+val rc_base (o1 o2:op_t)
+  : Lemma (requires Fst_then_snd? (rc o1 o2) /\ distinct_ops o1 o2)
+          (ensures eq (merge init_st (do init_st o1) (do init_st o2)) (do (do init_st o1) o2))
+
+val rc_inter_base_right_s (l a b c:concrete_st_s) (o1 o2 ob ol:op_s)
+  : Lemma (requires rc_s o1 o2 <> Either /\ rc_s ob ol <> Either /\ 
+                    distinct_ops o1 o2 /\ distinct_ops o1 ob /\ distinct_ops o1 ol /\ distinct_ops o2 ob /\ distinct_ops o2 ol /\ distinct_ops ob ol /\ 
+                    eq_s (merge_s (do_s l ol) (do_s (do_s a ol) o1) (do_s (do_s b ol) o2)) (do_s (do_s (do_s c ol) o1) o2) /\
+                    eq_s (merge_s l (do_s a o1) (do_s b o2)) (do_s (do_s c o1) o2) /\
+                    eq_s (merge_s l (do_s a ol) (do_s b ob)) (do_s (do_s c ob) ol)) //***EXTRA***
+          (ensures eq_s (merge_s (do_s l ol) (do_s (do_s a ol) o1) (do_s (do_s (do_s b ob) ol) o2)) (do_s (do_s (do_s (do_s c ob) ol) o1) o2))
+
+val rc_inter_base_right_ne (l a b c:concrete_st) (o1 o2 ob ol:op_t) 
+  : Lemma (requires Fst_then_snd? (rc o1 o2) /\ Fst_then_snd? (rc ob ol) /\ 
+                    distinct_ops o1 o2 /\ distinct_ops o1 ob /\ distinct_ops o1 ol /\ distinct_ops o2 ob /\ distinct_ops o2 ol /\ distinct_ops ob ol /\ 
+                    ~ (get_key o1 = get_key o2 /\ get_key o2 = get_key ob) /\
+                    eq (merge (do l ol) (do (do a ol) o1) (do (do b ol) o2)) (do (do (do c ol) o1) o2) /\
+                    eq (merge l (do a o1) (do b o2)) (do (do c o1) o2) /\
+                    eq (merge l (do a ol) (do b ob)) (do (do c ob) ol)) //***EXTRA***
+          (ensures eq (merge (do l ol) (do (do a ol) o1) (do (do (do b ob) ol) o2)) (do (do (do (do c ob) ol) o1) o2))
+          
+let rc_inter_base_right (l a b c:concrete_st) (o1 o2 ob ol:op_t) 
+  : Lemma (requires Fst_then_snd? (rc o1 o2) /\ Fst_then_snd? (rc ob ol) /\ 
+                    distinct_ops o1 o2 /\ distinct_ops o1 ob /\ distinct_ops o1 ol /\ distinct_ops o2 ob /\ distinct_ops o2 ol /\ distinct_ops ob ol /\ 
+                    eq (merge (do l ol) (do (do a ol) o1) (do (do b ol) o2)) (do (do (do c ol) o1) o2) /\
+                    eq (merge l (do a o1) (do b o2)) (do (do c o1) o2) /\
+                    eq (merge l (do a ol) (do b ob)) (do (do c ob) ol)) //***EXTRA***
+          (ensures eq (merge (do l ol) (do (do a ol) o1) (do (do (do b ob) ol) o2)) (do (do (do (do c ob) ol) o1) o2)) =
+  let k = get_key ob in
+  let l' = sel l k in let a' = sel a k in let b' = sel b k in let c' = sel c k in
+  if get_key o2 = get_key o1 && get_key o1 = k then 
+    rc_inter_base_right_s l' a' b' c' (get_op_s o1) (get_op_s o2) (get_op_s ob) (get_op_s ol)
+  else rc_inter_base_right_ne l a b c o1 o2 ob ol
+
+val rc_inter_base_left_s (l a b c:concrete_st_s) (o1 o2 ob ol:op_s)
+  : Lemma (requires rc_s o1 o2 <> Either /\ rc_s ob ol <> Either /\ 
+                    distinct_ops o1 o2 /\ distinct_ops o1 ob /\ distinct_ops o1 ol /\ distinct_ops o2 ob /\ distinct_ops o2 ol /\ distinct_ops ob ol /\ 
+                    eq_s (merge_s (do_s l ol) (do_s (do_s a ol) o1) (do_s (do_s b ol) o2)) (do_s (do_s (do_s c ol) o1) o2) /\
+                    eq_s (merge_s l (do_s a o1) (do_s b o2)) (do_s (do_s c o1) o2) /\
+                    eq_s (merge_s l (do_s a ob) (do_s b ol)) (do_s (do_s c ob) ol)) //***EXTRA***
+          (ensures eq_s (merge_s (do_s l ol) (do_s (do_s (do_s a ob) ol) o1) (do_s (do_s b ol) o2)) (do_s (do_s (do_s (do_s c ob) ol) o1) o2))
+
+val rc_inter_base_left_ne (l a b c:concrete_st) (o1 o2 ob ol:op_t) 
+  : Lemma (requires Fst_then_snd? (rc o1 o2) /\ Fst_then_snd? (rc ob ol) /\ 
+                    distinct_ops o1 o2 /\ distinct_ops o1 ob /\ distinct_ops o1 ol /\ distinct_ops o2 ob /\ distinct_ops o2 ol /\ distinct_ops ob ol /\ 
+                    ~ (get_key o1 = get_key o2 /\ get_key o2 = get_key ob) /\
+                    eq (merge (do l ol) (do (do a ol) o1) (do (do b ol) o2)) (do (do (do c ol) o1) o2) /\
+                    eq (merge l (do a o1) (do b o2)) (do (do c o1) o2) /\
+                    eq (merge l (do a ob) (do b ol)) (do (do c ob) ol)) //***EXTRA***
+          (ensures eq (merge (do l ol) (do (do (do a ob) ol) o1) (do (do b ol) o2)) (do (do (do (do c ob) ol) o1) o2))
+          
+let rc_inter_base_left (l a b c:concrete_st) (o1 o2 ob ol:op_t) 
+  : Lemma (requires Fst_then_snd? (rc o1 o2) /\ Fst_then_snd? (rc ob ol) /\ 
+                    distinct_ops o1 o2 /\ distinct_ops o1 ob /\ distinct_ops o1 ol /\ distinct_ops o2 ob /\ distinct_ops o2 ol /\ distinct_ops ob ol /\ 
+                    eq (merge (do l ol) (do (do a ol) o1) (do (do b ol) o2)) (do (do (do c ol) o1) o2) /\
+                    eq (merge l (do a o1) (do b o2)) (do (do c o1) o2) /\
+                    eq (merge l (do a ob) (do b ol)) (do (do c ob) ol)) //***EXTRA***
+          (ensures eq (merge (do l ol) (do (do (do a ob) ol) o1) (do (do b ol) o2)) (do (do (do (do c ob) ol) o1) o2)) =
+  let k = get_key ob in
+  let l' = sel l k in let a' = sel a k in let b' = sel b k in let c' = sel c k in
+  if get_key o2 = get_key o1 && get_key o1 = k then 
+    rc_inter_base_left_s l' a' b' c' (get_op_s o1) (get_op_s o2) (get_op_s ob) (get_op_s ol)
+  else rc_inter_base_left_ne l a b c o1 o2 ob ol
+
+val rc_inter_right_s (l a b c:concrete_st_s) (o1 o2 ob ol o:op_s)
+  : Lemma (requires rc_s o1 o2 <> Either /\ rc_s ob ol <> Either /\ 
+                    distinct_ops o1 o2 /\ distinct_ops o1 ob /\ distinct_ops o1 ol /\ distinct_ops o1 o /\ distinct_ops o2 ob /\ 
+                    distinct_ops o2 ol /\ distinct_ops o2 o /\ distinct_ops ob ol /\ distinct_ops ob o /\ distinct_ops ol o /\
+                    get_rid o <> get_rid ol /\
+                    eq_s (merge_s (do_s l ol) (do_s (do_s a ol) o1) (do_s (do_s (do_s b ob) ol) o2)) (do_s (do_s (do_s (do_s c ob) ol) o1) o2))
+      (ensures eq_s (merge_s (do_s l ol) (do_s (do_s a ol) o1) (do_s (do_s (do_s (do_s b o) ob) ol) o2)) (do_s (do_s (do_s (do_s (do_s c o) ob) ol) o1) o2))
+
+val rc_inter_right_ne (l a b c:concrete_st) (o1 o2 ob ol o:op_t) 
+  : Lemma (requires Fst_then_snd? (rc o1 o2) /\ Fst_then_snd? (rc ob ol) /\ 
+                    distinct_ops o1 o2 /\ distinct_ops o1 ob /\ distinct_ops o1 ol /\ distinct_ops o1 o /\ distinct_ops o2 ob /\ 
+                    distinct_ops o2 ol /\ distinct_ops o2 o /\ distinct_ops ob ol /\ distinct_ops ob o /\ distinct_ops ol o /\
+                    ~ (get_key o1 = get_key o2 /\ get_key o2 = get_key ob) /\
+                    get_rid o <> get_rid ol (*o,ol must be concurrent*) /\
+                    ((~ (commutes_with o ob)) \/ Fst_then_snd? (rc o ol)) /\
+                    eq (merge (do l ol) (do (do a ol) o1) (do (do (do b ob) ol) o2)) (do (do (do (do c ob) ol) o1) o2))
+      (ensures eq (merge (do l ol) (do (do a ol) o1) (do (do (do (do b o) ob) ol) o2)) (do (do (do (do (do c o) ob) ol) o1) o2))
+          
+let rc_inter_right (l a b c:concrete_st) (o1 o2 ob ol o:op_t)
+  : Lemma (requires Fst_then_snd? (rc o1 o2) /\ Fst_then_snd? (rc ob ol) /\ 
+                    distinct_ops o1 o2 /\ distinct_ops o1 ob /\ distinct_ops o1 ol /\ distinct_ops o1 o /\ distinct_ops o2 ob /\ 
+                    distinct_ops o2 ol /\ distinct_ops o2 o /\ distinct_ops ob ol /\ distinct_ops ob o /\ distinct_ops ol o /\
+                    get_rid o <> get_rid ol (*o,ol must be concurrent*) /\
+                    ((~ (commutes_with o ob)) \/ Fst_then_snd? (rc o ol)) /\
+                    eq (merge (do l ol) (do (do a ol) o1) (do (do (do b ob) ol) o2)) (do (do (do (do c ob) ol) o1) o2))
+      (ensures eq (merge (do l ol) (do (do a ol) o1) (do (do (do (do b o) ob) ol) o2)) (do (do (do (do (do c o) ob) ol) o1) o2)) =
+  let k = get_key o in
+  let l' = sel l k in let a' = sel a k in let b' = sel b k in let c' = sel c k in
+  if get_key o2 = get_key o1 && get_key o1 = k then 
+    rc_inter_right_s l' a' b' c' (get_op_s o1) (get_op_s o2) (get_op_s ob) (get_op_s ol) (get_op_s o)
+  else rc_inter_right_ne l a b c o1 o2 ob ol o
+
+val rc_inter_left_s (l a b c:concrete_st_s) (o1 o2 ob ol o:op_s)
+  : Lemma (requires rc_s o1 o2 <> Either /\ rc_s ob ol <> Either /\ 
+                    distinct_ops o1 o2 /\ distinct_ops o1 ob /\ distinct_ops o1 ol /\ distinct_ops o1 o /\ distinct_ops o2 ob /\ 
+                    distinct_ops o2 ol /\ distinct_ops o2 o /\ distinct_ops ob ol /\ distinct_ops ob o /\ distinct_ops ol o /\
+                    get_rid o <> get_rid ol /\
+                    eq_s (merge_s (do_s l ol) (do_s (do_s (do_s a ob) ol) o1) (do_s (do_s b ol) o2)) (do_s (do_s (do_s (do_s c ob) ol) o1) o2))
+      (ensures eq_s (merge_s (do_s l ol) (do_s (do_s (do_s (do_s a o) ob) ol) o1) (do_s (do_s b ol) o2)) (do_s (do_s (do_s (do_s (do_s c o) ob) ol) o1) o2))
+
+val rc_inter_left_ne (l a b c:concrete_st) (o1 o2 ob ol o:op_t) 
+  : Lemma (requires Fst_then_snd? (rc o1 o2) /\ Fst_then_snd? (rc ob ol) /\ 
+                    distinct_ops o1 o2 /\ distinct_ops o1 ob /\ distinct_ops o1 ol /\ distinct_ops o1 o /\ distinct_ops o2 ob /\ 
+                    distinct_ops o2 ol /\ distinct_ops o2 o /\ distinct_ops ob ol /\ distinct_ops ob o /\ distinct_ops ol o /\
+                    ~ (get_key o1 = get_key o2 /\ get_key o2 = get_key ob) /\
+                    get_rid o <> get_rid ol (*o,ol must be concurrent*) /\
+                    ((~ (commutes_with o ob)) \/ Fst_then_snd? (rc o ol)) /\
+                    eq (merge (do l ol) (do (do (do a ob) ol) o1) (do (do b ol) o2)) (do (do (do (do c ob) ol) o1) o2))
+      (ensures eq (merge (do l ol) (do (do (do (do a o) ob) ol) o1) (do (do b ol) o2)) (do (do (do (do (do c o) ob) ol) o1) o2))
+      
+let rc_inter_left (l a b c:concrete_st) (o1 o2 ob ol o:op_t)
+  : Lemma (requires Fst_then_snd? (rc o1 o2) /\ Fst_then_snd? (rc ob ol) /\ 
+                    distinct_ops o1 o2 /\ distinct_ops o1 ob /\ distinct_ops o1 ol /\ distinct_ops o1 o /\ distinct_ops o2 ob /\ 
+                    distinct_ops o2 ol /\ distinct_ops o2 o /\ distinct_ops ob ol /\ distinct_ops ob o /\ distinct_ops ol o /\
+                    get_rid o <> get_rid ol (*o,ol must be concurrent*) /\
+                    ((~ (commutes_with o ob)) \/ Fst_then_snd? (rc o ol)) /\
+                    eq (merge (do l ol) (do (do (do a ob) ol) o1) (do (do b ol) o2)) (do (do (do (do c ob) ol) o1) o2))
+      (ensures eq (merge (do l ol) (do (do (do (do a o) ob) ol) o1) (do (do b ol) o2)) (do (do (do (do (do c o) ob) ol) o1) o2)) =
+  let k = get_key o in
+  let l' = sel l k in let a' = sel a k in let b' = sel b k in let c' = sel c k in
+  if get_key o2 = get_key o1 && get_key o1 = k then 
+    rc_inter_left_s l' a' b' c' (get_op_s o1) (get_op_s o2) (get_op_s ob) (get_op_s ol) (get_op_s o)
+  else rc_inter_left_ne l a b c o1 o2 ob ol o
+
+val rc_inter_lca_s (l a b c:concrete_st_s) (o1 o2 ol oi:op_s)
+  : Lemma (requires rc_s o1 o2 <> Either /\ 
+                    distinct_ops o1 o2 /\ distinct_ops o1 ol /\ distinct_ops o1 oi /\ distinct_ops o2 ol /\ distinct_ops o2 oi /\ distinct_ops ol oi /\
+                    (exists o. rc_s o ol <> Either) /\ 
+                    (exists o. rc_s o oi <> Either) /\
+                    eq_s (merge_s (do_s l oi) (do_s (do_s a oi) o1) (do_s (do_s b oi) o2)) (do_s (do_s (do_s c oi) o1) o2) /\
+                    eq_s (merge_s (do_s l ol) (do_s (do_s a ol) o1) (do_s (do_s b ol) o2)) (do_s (do_s (do_s c ol) o1) o2))
+    (ensures eq_s (merge_s (do_s (do_s l oi) ol) (do_s (do_s (do_s a oi) ol) o1) (do_s (do_s (do_s b oi) ol) o2)) (do_s (do_s (do_s (do_s c oi) ol) o1) o2))
+
+val rc_inter_lca_ne (l a b c:concrete_st) (o1 o2 ol oi:op_t) 
+  : Lemma (requires Fst_then_snd? (rc o1 o2) /\ 
+                    distinct_ops o1 o2 /\ distinct_ops o1 ol /\ distinct_ops o1 oi /\ distinct_ops o2 ol /\ distinct_ops o2 oi /\ distinct_ops ol oi /\
+                    ~ (get_key o1 = get_key o2 /\ get_key o1 = get_key oi /\ get_key o1 = get_key ol) /\
+                    
+                    (exists o. Fst_then_snd? (rc o ol)) /\ 
+                    (exists o. Fst_then_snd? (rc o oi)) /\ 
+                    eq (merge (do l oi) (do (do a oi) o1) (do (do b oi) o2)) (do (do (do c oi) o1) o2) /\
+                    eq (merge (do l ol) (do (do a ol) o1) (do (do b ol) o2)) (do (do (do c ol) o1) o2))
+    (ensures eq (merge (do (do l oi) ol) (do (do (do a oi) ol) o1) (do (do (do b oi) ol) o2)) (do (do (do (do c oi) ol) o1) o2))
+      
+// In general, the events ol,oi, below should be such that these exists o, (rc o ol), (rc o oi)
+let rc_inter_lca (l a b c:concrete_st) (o1 o2 ol oi:op_t)
+  : Lemma (requires Fst_then_snd? (rc o1 o2) /\ 
+                    distinct_ops o1 o2 /\ distinct_ops o1 ol /\ distinct_ops o1 oi /\ distinct_ops o2 ol /\ distinct_ops o2 oi /\ distinct_ops ol oi /\
+                    (exists o. Fst_then_snd? (rc o ol)) /\ 
+                    (exists o. Fst_then_snd? (rc o oi)) /\ 
+                    eq (merge (do l oi) (do (do a oi) o1) (do (do b oi) o2)) (do (do (do c oi) o1) o2) /\
+                    eq (merge (do l ol) (do (do a ol) o1) (do (do b ol) o2)) (do (do (do c ol) o1) o2))
+    (ensures eq (merge (do (do l oi) ol) (do (do (do a oi) ol) o1) (do (do (do b oi) ol) o2)) (do (do (do (do c oi) ol) o1) o2)) =
+  let k = get_key oi in
+  let l' = sel l k in let a' = sel a k in let b' = sel b k in let c' = sel c k in
+  if get_key o2 = get_key o1 && get_key o1 = k && get_key o1 = get_key ol then 
+    rc_inter_lca_s l' a' b' c' (get_op_s o1) (get_op_s o2) (get_op_s ol) (get_op_s oi)
+  else rc_inter_lca_ne l a b c o1 o2 ol oi
+
+(*One op*)
+///////////////
+val one_op_ind_right_s (l a b:concrete_st_s) (o2 o2':op_s) 
+  : Lemma (requires distinct_ops o2 o2' /\ 
+                    eq_s (merge_s l a (do_s b o2)) (do_s (merge_s l a b) o2))
+           (ensures eq_s (merge_s l a (do_s (do_s b o2') o2)) (do_s (merge_s l a (do_s b o2')) o2))
+
+val one_op_ind_right_ne (l a b:concrete_st) (o2 o2':op_t)
+  : Lemma (requires distinct_ops o2 o2' /\ 
+                    ~ (get_key o2 = get_key o2') /\
+                    eq (merge l a (do b o2)) (do (merge l a b) o2))
+           (ensures eq (merge l a (do (do b o2') o2)) (do (merge l a (do b o2')) o2))
+
+let one_op_ind_right (l a b:concrete_st) (o2 o2':op_t)
+   : Lemma (requires distinct_ops o2 o2' /\ eq (merge l a (do b o2)) (do (merge l a b) o2))
+           (ensures eq (merge l a (do (do b o2') o2)) (do (merge l a (do b o2')) o2)) =
+  let k = get_key o2' in
+  let l' = sel l k in let a' = sel a k in let b' = sel b k in 
+  lemma_merge l a b;
+  if get_key o2 = k then
+   one_op_ind_right_s l' a' b' (get_op_s o2) (get_op_s o2')
+  else one_op_ind_right_ne l a b o2 o2'
+
+val one_op_ind_left_s (l a b:concrete_st_s) (o1 o1':op_s) 
+  : Lemma (requires distinct_ops o1 o1' /\ 
+                    eq_s (merge_s l (do_s a o1) b) (do_s (merge_s l a b) o1))
+           (ensures eq_s (merge_s l (do_s (do_s a o1') o1) b) (do_s (merge_s l (do_s a o1') b) o1))
+
+val one_op_ind_left_ne (l a b:concrete_st) (o1 o1':op_t)
+   : Lemma (requires distinct_ops o1 o1' /\ 
+                     ~ (get_key o1 = get_key o1') /\
+                    eq (merge l (do a o1) b) (do (merge l a b) o1))
+           (ensures eq (merge l (do (do a o1') o1) b) (do (merge l (do a o1') b) o1))
+
+let one_op_ind_left (l a b:concrete_st) (o1 o1':op_t)
+   : Lemma (requires distinct_ops o1 o1' /\ eq (merge l (do a o1) b) (do (merge l a b) o1))
+           (ensures eq (merge l (do (do a o1') o1) b) (do (merge l (do a o1') b) o1)) =
+  let k = get_key o1' in
+  let l' = sel l k in let a' = sel a k in let b' = sel b k in 
+  lemma_merge l a b;
+  if get_key o1 = k then
+   one_op_ind_left_s l' a' b' (get_op_s o1) (get_op_s o1')
+  else one_op_ind_left_ne l a b o1 o1'
+
+val one_op_ind_lca_s (l:concrete_st_s) (o2 o:op_s) 
+  : Lemma (requires distinct_ops o2 o /\ 
+                    eq_s (merge_s l l (do_s l o2)) (do_s l o2))
+          (ensures eq_s (merge_s (do_s l o) (do_s l o) (do_s (do_s l o) o2)) (do_s (do_s l o) o2)) 
+
+val one_op_ind_lca_ne (l:concrete_st) (o2 o:op_t)
+   : Lemma (requires distinct_ops o2 o /\ 
+                     ~ (get_key o2 = get_key o) /\
+                     eq (merge l l (do l o2)) (do l o2))
+          (ensures eq (merge (do l o) (do l o) (do (do l o) o2)) (do (do l o) o2)) 
+           
+let one_op_ind_lca (l:concrete_st) (o2 o:op_t)
+  : Lemma (requires distinct_ops o2 o /\ eq (merge l l (do l o2)) (do l o2))
+          (ensures eq (merge (do l o) (do l o) (do (do l o) o2)) (do (do l o) o2)) =
+  let k = get_key o in
+  let l' = sel l k in 
+  if get_key o2 = k then
+   one_op_ind_lca_s l' (get_op_s o2) (get_op_s o)
+  else one_op_ind_lca_ne l o2 o
+
+val one_op_base (o2:op_t)
+  : Lemma (ensures eq (merge init_st init_st (do init_st o2)) (do init_st o2))
+
+val one_op_inter_base_right_s (l a b c:concrete_st_s) (o2 ob ol:op_s)
+  : Lemma (requires rc_s ob ol <> Either /\ 
+                    distinct_ops o2 ob /\ distinct_ops o2 ol /\ distinct_ops ob ol /\ 
+                    eq_s (merge_s (do_s l ol) (do_s a ol) (do_s (do_s b ol) o2)) (do_s (do_s c ol) o2) /\
+                    eq_s (merge_s l a (do_s b o2)) (do_s c o2) /\
+                    eq_s (merge_s l (do_s a ol) (do_s b ob)) (do_s (do_s c ob) ol)) //***EXTRA***
+          (ensures eq_s (merge_s (do_s l ol) (do_s a ol) (do_s (do_s (do_s b ob) ol) o2)) (do_s (do_s (do_s c ob) ol) o2))
+
+val one_op_inter_base_right_ne (l a b c:concrete_st) (o2 ob ol:op_t) 
+  : Lemma (requires Fst_then_snd? (rc ob ol) /\ 
+                    distinct_ops o2 ob /\ distinct_ops o2 ol /\ distinct_ops ob ol /\ 
+                    ~ (get_key o2 = get_key ob) /\
+                    eq (merge (do l ol) (do a ol) (do (do b ol) o2)) (do (do c ol) o2) /\
+                    eq (merge l a (do b o2)) (do c o2) /\
+                    eq (merge l (do a ol) (do b ob)) (do (do c ob) ol)) //***EXTRA***
+          (ensures eq (merge (do l ol) (do a ol) (do (do (do b ob) ol) o2)) (do (do (do c ob) ol) o2))
+          
+let one_op_inter_base_right (l a b c:concrete_st) (o2 ob ol:op_t) 
+  : Lemma (requires Fst_then_snd? (rc ob ol) /\
+                    distinct_ops o2 ob /\ distinct_ops o2 ol /\ distinct_ops ob ol /\
+                    eq (merge (do l ol) (do a ol) (do (do b ol) o2)) (do (do c ol) o2) /\
+                    eq (merge l a (do b o2)) (do c o2) /\
+                    eq (merge l (do a ol) (do b ob)) (do (do c ob) ol)) //***EXTRA***
+          (ensures eq (merge (do l ol) (do a ol) (do (do (do b ob) ol) o2)) (do (do (do c ob) ol) o2)) =
+  let k = get_key ob in
+  let l' = sel l k in let a' = sel a k in let b' = sel b k in let c' = sel c k in
+  if get_key o2 = get_key ob then
+    one_op_inter_base_right_s l' a' b' c' (get_op_s o2) (get_op_s ob) (get_op_s ol)
+  else one_op_inter_base_right_ne l a b c o2 ob ol
+
+val one_op_inter_base_left_s (l a b c:concrete_st_s) (o2 ob ol:op_s)
+  : Lemma (requires rc_s ob ol <> Either /\ 
+                    distinct_ops o2 ob /\ distinct_ops o2 ol /\ distinct_ops ob ol /\ 
+                    eq_s (merge_s (do_s l ol) (do_s a ol) (do_s (do_s b ol) o2)) (do_s (do_s c ol) o2) /\
+                    eq_s (merge_s l a (do_s b o2)) (do_s c o2) /\
+                    eq_s (merge_s l (do_s a ol) (do_s b ob)) (do_s (do_s c ob) ol) /\ //***EXTRA***
+                    eq_s (merge_s l (do_s (do_s a ob) ol) (do_s b ol)) (do_s (do_s c ob) ol)) //***EXTRA***
+          (ensures eq_s (merge_s (do_s l ol) (do_s (do_s a ob) ol) (do_s (do_s b ol) o2)) (do_s (do_s (do_s c ob) ol) o2))
+
+val one_op_inter_base_left_ne (l a b c:concrete_st) (o2 ob ol:op_t) 
+  : Lemma (requires Fst_then_snd? (rc ob ol) /\
+                    distinct_ops o2 ob /\ distinct_ops o2 ol /\ distinct_ops ob ol /\
+                    ~ (get_key o2 = get_key ob) /\
+                    eq (merge (do l ol) (do a ol) (do (do b ol) o2)) (do (do c ol) o2) /\
+                    (Fst_then_snd? (rc ob o2) ==> eq (merge l (do a o2) (do b ob)) (do (merge l a (do b ob)) o2)) /\ //***EXTRA***
+                    eq (merge l a (do b o2)) (do c o2) /\
+                    eq (merge l (do a ol) (do b ob)) (do (do c ob) ol) /\ //***EXTRA***
+                    eq (merge l (do (do a ob) ol) (do b ol)) (do (do c ob) ol)) //***EXTRA***
+          (ensures eq (merge (do l ol) (do (do a ob) ol) (do (do b ol) o2)) (do (do (do c ob) ol) o2))
+          
+let one_op_inter_base_left (l a b c:concrete_st) (o2 ob ol:op_t) 
+  : Lemma (requires Fst_then_snd? (rc ob ol) /\
+                    distinct_ops o2 ob /\ distinct_ops o2 ol /\ distinct_ops ob ol /\
+                    eq (merge (do l ol) (do a ol) (do (do b ol) o2)) (do (do c ol) o2) /\
+                    (Fst_then_snd? (rc ob o2) ==> eq (merge l (do a o2) (do b ob)) (do (merge l a (do b ob)) o2)) /\ //***EXTRA***
+                    eq (merge l a (do b o2)) (do c o2) /\
+                    eq (merge l (do a ol) (do b ob)) (do (do c ob) ol) /\ //***EXTRA***
+                    eq (merge l (do (do a ob) ol) (do b ol)) (do (do c ob) ol)) //***EXTRA***
+          (ensures eq (merge (do l ol) (do (do a ob) ol) (do (do b ol) o2)) (do (do (do c ob) ol) o2)) =
+  let k = get_key ob in
+  let l' = sel l k in let a' = sel a k in let b' = sel b k in let c' = sel c k in
+  if get_key o2 = get_key ob then
+    one_op_inter_base_left_s l' a' b' c' (get_op_s o2) (get_op_s ob) (get_op_s ol)
+  else one_op_inter_base_left_ne l a b c o2 ob ol
+
+val one_op_inter_right_s (l a b c:concrete_st_s) (o2 ob ol o:op_s)
+  : Lemma (requires rc_s ob ol <> Either /\ 
+                    distinct_ops o ob /\ distinct_ops o ol /\ distinct_ops o o2 /\ distinct_ops ob ol /\ distinct_ops ob o2 /\ distinct_ops o2 ol /\
+                    get_rid o <> get_rid ol /\
+                    eq_s (merge_s (do_s l ol) (do_s a ol) (do_s (do_s (do_s b ob) ol) o2)) (do_s (do_s (do_s c ob) ol) o2))
+      (ensures eq_s (merge_s (do_s l ol) (do_s a ol) (do_s (do_s (do_s (do_s b o) ob) ol) o2)) (do_s (do_s (do_s (do_s c o) ob) ol) o2))
+
+val one_op_inter_right_ne (l a b c:concrete_st) (o2 ob ol o:op_t) 
+  : Lemma (requires Fst_then_snd? (rc ob ol) /\
+                    distinct_ops o ob /\ distinct_ops o ol /\ distinct_ops o o2 /\ distinct_ops ob ol /\ distinct_ops ob o2 /\ distinct_ops o2 ol /\
+                    ~ (get_key o2 = get_key ob) /\
+                    get_rid o <> get_rid ol (*o,ol must be concurrent*) /\
+                    ((~ (commutes_with o ob)) \/ Fst_then_snd? (rc o ol)) /\
+                    eq (merge (do l ol) (do a ol) (do (do (do b ob) ol) o2)) (do (do (do c ob) ol) o2))
+          (ensures eq (merge (do l ol) (do a ol) (do (do (do (do b o) ob) ol) o2)) (do (do (do (do c o) ob) ol) o2))
+      
+let one_op_inter_right (l a b c:concrete_st) (o2 ob ol o:op_t) 
+  : Lemma (requires Fst_then_snd? (rc ob ol) /\
+                    distinct_ops o ob /\ distinct_ops o ol /\ distinct_ops o o2 /\ distinct_ops ob ol /\ distinct_ops ob o2 /\ distinct_ops o2 ol /\
+                    get_rid o <> get_rid ol (*o,ol must be concurrent*) /\
+                    ((~ (commutes_with o ob)) \/ Fst_then_snd? (rc o ol)) /\
+                    eq (merge (do l ol) (do a ol) (do (do (do b ob) ol) o2)) (do (do (do c ob) ol) o2))
+          (ensures eq (merge (do l ol) (do a ol) (do (do (do (do b o) ob) ol) o2)) (do (do (do (do c o) ob) ol) o2)) =
+  let k = get_key o in
+  let l' = sel l k in let a' = sel a k in let b' = sel b k in let c' = sel c k in
+  if get_key o2 = get_key ob then 
+    one_op_inter_right_s l' a' b' c' (get_op_s o2) (get_op_s ob) (get_op_s ol) (get_op_s o)
+  else one_op_inter_right_ne l a b c o2 ob ol o
+
+val one_op_inter_left_s (l a b c:concrete_st_s) (o2 ob ol o:op_s)
+  : Lemma (requires rc_s ob ol <> Either /\ 
+                    distinct_ops o ob /\ distinct_ops o ol /\ distinct_ops o o2 /\ distinct_ops ob ol /\ distinct_ops ob o2 /\ distinct_ops o2 ol /\
+                    get_rid o <> get_rid ol /\
+                    eq_s (merge_s (do_s l ol) (do_s (do_s a ob) ol) (do_s (do_s b ol) o2)) (do_s (do_s (do_s c ob) ol) o2))
+          (ensures eq_s (merge_s (do_s l ol) (do_s (do_s (do_s a o) ob) ol) (do_s (do_s b ol) o2)) (do_s (do_s (do_s (do_s c o) ob) ol) o2))
+
+val one_op_inter_left_ne (l a b c:concrete_st) (o2 ob ol o:op_t) 
+  : Lemma (requires Fst_then_snd? (rc ob ol) /\
+                    distinct_ops o ob /\ distinct_ops o ol /\ distinct_ops o ol /\ distinct_ops ob ol /\ distinct_ops ob o2 /\ distinct_ops o2 ol /\
+                    ~ (get_key o2 = get_key ob) /\
+                    get_rid o <> get_rid ol (*o,ol must be concurrent*) /\
+                    ((~ (commutes_with o ob)) \/ Fst_then_snd? (rc o ol)) /\
+                    eq (merge (do l ol) (do (do a ob) ol) (do (do b ol) o2)) (do (do (do c ob) ol) o2))
+          (ensures eq (merge (do l ol) (do (do (do a o) ob) ol) (do (do b ol) o2)) (do (do (do (do c o) ob) ol) o2))
+          
+let one_op_inter_left (l a b c:concrete_st) (o2 ob ol o:op_t) 
+  : Lemma (requires Fst_then_snd? (rc ob ol) /\
+                    distinct_ops o ob /\ distinct_ops o ol /\ distinct_ops o o2 /\ distinct_ops ob ol /\ distinct_ops ob o2 /\ distinct_ops o2 ol /\
+                    get_rid o <> get_rid ol (*o,ol must be concurrent*) /\
+                    ((~ (commutes_with o ob)) \/ Fst_then_snd? (rc o ol)) /\
+                    eq (merge (do l ol) (do (do a ob) ol) (do (do b ol) o2)) (do (do (do c ob) ol) o2))
+          (ensures eq (merge (do l ol) (do (do (do a o) ob) ol) (do (do b ol) o2)) (do (do (do (do c o) ob) ol) o2)) =
+  let k = get_key o in
+  let l' = sel l k in let a' = sel a k in let b' = sel b k in let c' = sel c k in
+  if get_key o2 = get_key ob then 
+    one_op_inter_left_s l' a' b' c' (get_op_s o2) (get_op_s ob) (get_op_s ol) (get_op_s o)
+  else one_op_inter_left_ne l a b c o2 ob ol o
+
+val one_op_inter_lca_s (l a b c:concrete_st_s) (o2 ol oi:op_s)
+  : Lemma (requires distinct_ops o2 ol /\ distinct_ops o2 oi /\ distinct_ops ol oi /\ 
+                    (exists o. rc_s o ol <> Either) /\ 
+                    (exists o. rc_s o oi <> Either) /\
+                    eq_s (merge_s (do_s l oi) (do_s a oi) (do_s (do_s b oi) o2)) (do_s (do_s c oi) o2) /\
+                    eq_s (merge_s (do_s l ol) (do_s a ol) (do_s (do_s b ol) o2)) (do_s (do_s c ol) o2))
+    (ensures eq_s (merge_s (do_s (do_s l oi) ol) (do_s (do_s a oi) ol) (do_s (do_s (do_s b oi) ol) o2)) (do_s (do_s (do_s c oi) ol) o2))
+
+val one_op_inter_lca_ne (l a b c:concrete_st) (o2 ol oi:op_t)
+  : Lemma (requires distinct_ops o2 ol /\ distinct_ops o2 oi /\ distinct_ops ol oi /\ 
+                    ~ (get_key o2 = get_key oi /\ get_key o2 = get_key ol) /\
+                    (exists o. Fst_then_snd? (rc o ol)) /\ 
+                    (exists o. Fst_then_snd? (rc o oi)) /\ 
+                    eq (merge (do l oi) (do a oi) (do (do b oi) o2)) (do (do c oi) o2) /\
+                    eq (merge (do l ol) (do a ol) (do (do b ol) o2)) (do (do c ol) o2))
+          (ensures eq (merge (do (do l oi) ol) (do (do a oi) ol) (do (do (do b oi) ol) o2)) (do (do (do c oi) ol) o2))
+  
+// In general, the events o',o_n, below should be such that these exists o, (rc o o')
+let one_op_inter_lca (l a b c:concrete_st) (o2 ol oi:op_t)
+  : Lemma (requires distinct_ops o2 ol /\ distinct_ops o2 oi /\ distinct_ops ol oi /\ 
+                    (exists o. Fst_then_snd? (rc o ol)) /\ 
+                    (exists o. Fst_then_snd? (rc o oi)) /\ 
+                    eq (merge (do l oi) (do a oi) (do (do b oi) o2)) (do (do c oi) o2) /\
+                    eq (merge (do l ol) (do a ol) (do (do b ol) o2)) (do (do c ol) o2))
+          (ensures eq (merge (do (do l oi) ol) (do (do a oi) ol) (do (do (do b oi) ol) o2)) (do (do (do c oi) ol) o2)) =
+  let k = get_key oi in
+  let l' = sel l k in let a' = sel a k in let b' = sel b k in let c' = sel c k in
+  if get_key o2 = k && get_key o2 = get_key ol then 
+    one_op_inter_lca_s l' a' b' c' (get_op_s o2) (get_op_s ol) (get_op_s oi)
+  else one_op_inter_lca_ne l a b c o2 ol oi
+
+(*Zero op *)
+///////////////
+val zero_op_inter_base_right_s (l a b c:concrete_st_s) (ob ol:op_s)
+  : Lemma (requires rc_s ob ol <> Either /\ distinct_ops ob ol /\ 
+                    eq_s (merge_s (do_s l ol) (do_s a ol) (do_s b ol)) (do_s c ol) /\
+                    eq_s (merge_s l a b) c /\
+                    eq_s (merge_s l (do_s a ol) (do_s b ob)) (do_s (do_s c ob) ol)) //***EXTRA***
+          (ensures eq_s (merge_s (do_s l ol) (do_s a ol) (do_s (do_s b ob) ol)) (do_s (do_s c ob) ol))
+
+// because we proved that e_i^l rcp eb is not possible.
+//e_i^l vis eb is not possible
+// so either eb rcp e_i^l or eb rct e_i^l is possible
+let zero_op_inter_base_right (l a b c:concrete_st) (ob ol:op_t) 
+  : Lemma (requires Fst_then_snd? (rc ob ol) /\ distinct_ops ob ol /\ 
+                    eq (merge (do l ol) (do a ol) (do b ol)) (do c ol) /\
+                    eq (merge l a b) c /\
+                    eq (merge l (do a ol) (do b ob)) (do (do c ob) ol)) //***EXTRA***
+          (ensures eq (merge (do l ol) (do a ol) (do (do b ob) ol)) (do (do c ob) ol)) =
+  let k = get_key ob in
+  let l' = sel l k in let a' = sel a k in let b' = sel b k in let c' = sel c k in
+  lemma_merge l a b;
+  zero_op_inter_base_right_s l' a' b' c' (get_op_s ob) (get_op_s ol)
+
+val zero_op_inter_base_left_s (l a b c:concrete_st_s) (ob ol:op_s)
+  : Lemma (requires rc_s ob ol <> Either /\ distinct_ops ob ol /\ 
+                    eq_s (merge_s (do_s l ol) (do_s a ol) (do_s b ol)) (do_s c ol) /\
+                    eq_s (merge_s l a b) c /\
+                    eq_s (merge_s l (do_s a ob) (do_s b ol)) (do_s (do_s c ob) ol)) //***EXTRA***
+          (ensures eq_s (merge_s (do_s l ol) (do_s (do_s a ob) ol) (do_s b ol)) (do_s (do_s c ob) ol))
+          
+let zero_op_inter_base_left (l a b c:concrete_st) (ob ol:op_t) 
+  : Lemma (requires Fst_then_snd? (rc ob ol) /\ distinct_ops ob ol /\ 
+                    eq (merge (do l ol) (do a ol) (do b ol)) (do c ol) /\
+                    eq (merge l a b) c /\
+                    eq (merge l (do a ob) (do b ol)) (do (do c ob) ol)) //***EXTRA***
+          (ensures eq (merge (do l ol) (do (do a ob) ol) (do b ol) ) (do (do c ob) ol)) =
+  let k = get_key ob in
+  let l' = sel l k in let a' = sel a k in let b' = sel b k in let c' = sel c k in
+  lemma_merge l a b;
+  zero_op_inter_base_left_s l' a' b' c' (get_op_s ob) (get_op_s ol)
+
+val zero_op_inter_right_s (l a b c:concrete_st_s) (ob ol o:op_s)
+  : Lemma (requires rc_s ob ol <> Either /\ distinct_ops ob ol /\ distinct_ops ob o /\ distinct_ops ol o /\
+                    get_rid o <> get_rid ol (*o,ol must be concurrent*) /\
+                    eq_s (merge_s (do_s l ol) (do_s a ol) (do_s (do_s b ob) ol)) (do_s (do_s c ob) ol))
+          (ensures eq_s (merge_s (do_s l ol) (do_s a ol) (do_s (do_s (do_s b o) ob) ol)) (do_s (do_s (do_s c o) ob) ol)) 
+          
+let zero_op_inter_right (l a b c:concrete_st) (ob ol o:op_t)
+  : Lemma (requires Fst_then_snd? (rc ob ol) /\ 
+                    distinct_ops ob ol /\ distinct_ops ob o /\ distinct_ops ol o /\
+                    get_rid o <> get_rid ol (*o,ol must be concurrent*) /\
+                    ((~ (commutes_with o ob)) \/ Fst_then_snd? (rc o ol)) /\
+                    eq (merge (do l ol) (do a ol) (do (do b ob) ol)) (do (do c ob) ol))
+          (ensures eq (merge (do l ol) (do a ol) (do (do (do b o) ob) ol)) (do (do (do c o) ob) ol)) =
+  let k = get_key ob in
+  let l' = sel l k in let a' = sel a k in let b' = sel b k in let c' = sel c k in
+  zero_op_inter_right_s l' a' b' c' (get_op_s ob) (get_op_s ol) (get_op_s o)
+
+val zero_op_inter_left_s (l a b c:concrete_st_s) (ob ol o:op_s)
+  : Lemma (requires rc_s ob ol <> Either /\ distinct_ops ob ol /\ distinct_ops ob o /\ distinct_ops ol o /\
+                    get_rid o <> get_rid ol (*o,ol must be concurrent*) /\
+                    eq_s (merge_s (do_s l ol) (do_s (do_s a ob) ol) (do_s b ol)) (do_s (do_s c ob) ol))
+          (ensures eq_s (merge_s (do_s l ol) (do_s (do_s (do_s a o) ob) ol) (do_s b ol)) (do_s (do_s (do_s c o) ob) ol)) 
+          
+let zero_op_inter_left (l a b c:concrete_st) (ob ol o:op_t)
+  : Lemma (requires Fst_then_snd? (rc ob ol) /\ 
+                    distinct_ops ob ol /\ distinct_ops ob o /\ distinct_ops ol o /\
+                    get_rid o <> get_rid ol (*o,ol must be concurrent*) /\
+                    ((~ (commutes_with o ob)) \/ Fst_then_snd? (rc o ol)) /\
+                    eq (merge (do l ol) (do (do a ob) ol) (do b ol)) (do (do c ob) ol))
+          (ensures eq (merge (do l ol) (do (do (do a o) ob) ol) (do b ol)) (do (do (do c o) ob) ol)) =
+  let k = get_key ob in
+  let l' = sel l k in let a' = sel a k in let b' = sel b k in let c' = sel c k in
+  zero_op_inter_left_s l' a' b' c' (get_op_s ob) (get_op_s ol) (get_op_s o)
+
+val zero_op_inter_lca_v1_s (l a b c:concrete_st_s) (ol:op_s)
+  : Lemma (requires (exists o'. rc_s o' ol <> Either) /\ eq_s (merge_s l a b) c)
+          (ensures eq_s (merge_s (do_s l ol) (do_s a ol) (do_s b ol)) (do_s c ol))
+
+// In general, the event "o" below should be such that these exists o', (rc o' o)
+let zero_op_inter_lca_v1 (l a b c:concrete_st) (ol:op_t)
+  : Lemma (requires (exists o'. Fst_then_snd? (rc o' ol)) /\ eq (merge l a b) c)
+          (ensures eq (merge (do l ol) (do a ol) (do b ol)) (do c ol)) =
+  let k = get_key ol in
+  let l' = sel l k in let a' = sel a k in let b' = sel b k in let c' = sel c k in
+  lemma_merge l a b;
+  zero_op_inter_lca_v1_s l' a' b' c' (get_op_s ol)
+
+val zero_op_inter_lca_v2_s (l a b c:concrete_st_s) (ol oi:op_s)
+  : Lemma (requires distinct_ops ol oi /\
+                    (exists o. rc_s o ol <> Either) /\ 
+                    (exists o. rc_s o oi <> Either) /\ 
+                    eq_s (merge_s (do_s l oi) (do_s a oi) (do_s b oi)) (do_s c oi)  /\
+                    eq_s (merge_s (do_s l ol) (do_s a ol) (do_s b ol)) (do_s c ol))
+          (ensures eq_s (merge_s (do_s (do_s l oi) ol) (do_s (do_s a oi) ol) (do_s (do_s b oi) ol)) (do_s (do_s c oi) ol))
+
+val zero_op_inter_lca_v2_ne (l a b c:concrete_st) (ol oi:op_t)
+  : Lemma (requires distinct_ops ol oi /\
+                    ~ (get_key ol = get_key oi) /\
+                    (exists o. Fst_then_snd? (rc o ol)) /\ 
+                    (exists o. Fst_then_snd? (rc o oi)) /\
+                    eq (merge (do l oi) (do a oi) (do b oi)) (do c oi)  /\
+                    eq (merge (do l ol) (do a ol) (do b ol)) (do c ol))
+          (ensures eq (merge (do (do l oi) ol) (do (do a oi) ol) (do (do b oi) ol)) (do (do c oi) ol))
+
+// In general, the events o',o_n, below should be such that these exists o, (rc o o')
+let zero_op_inter_lca_v2 (l a b c:concrete_st) (ol oi:op_t)
+  : Lemma (requires distinct_ops ol oi /\
+                    (exists o. Fst_then_snd? (rc o ol)) /\ 
+                    (exists o. Fst_then_snd? (rc o oi)) /\
+                    eq (merge (do l oi) (do a oi) (do b oi)) (do c oi)  /\
+                    eq (merge (do l ol) (do a ol) (do b ol)) (do c ol))
+          (ensures eq (merge (do (do l oi) ol) (do (do a oi) ol) (do (do b oi) ol)) (do (do c oi) ol)) =
+  let k = get_key ol in
+  let l' = sel l k in let a' = sel a k in let b' = sel b k in let c' = sel c k in
+  if get_key oi = k then
+    zero_op_inter_lca_v2_s l' a' b' c' (get_op_s ol) (get_op_s oi)
+  else zero_op_inter_lca_v2_ne l a b c ol oi
+          
 (*Two OP COMM*)
 //////////////// 
 
 //simpler MRDT lemma (Already proved for Grows-only set)
-val comm_ind_right_s (l a b:concrete_st_s) (o1 o2' o2:(nat & (nat & op_s)))
-  : Lemma (requires Either? (rc_s o1 o2) /\
-                    eq_s (merge_s l (do_s a o1) (do_s b o2)) (do_s (do_s (merge_s l a b) o2) o1))
+val comm_ind_right_s (l a b:concrete_st_s) (o1 o2' o2:op_s)
+  : Lemma (requires eq_s (merge_s l (do_s a o1) (do_s b o2)) (do_s (do_s (merge_s l a b) o2) o1))
           (ensures eq_s (merge_s l (do_s a o1) (do_s (do_s b o2') o2)) (do_s (do_s (merge_s l a (do_s b o2')) o2) o1))
 
 val comm_ind_right_ne (l a b:concrete_st) (o1 o2' o2:op_t)
-  : Lemma (requires Either? (rc o1 o2) /\ Either? (rc_s (get_op_s o1) (get_op_s o2)) /\
+  : Lemma (requires Either? (rc o1 o2) /\
                      ~ (get_key o1 = get_key o2 /\ get_key o2 = get_key o2') /\
                     eq (merge l (do a o1) (do b o2)) (do (do (merge l a b) o2) o1))                    
           (ensures eq (merge l (do a o1) (do (do b o2') o2)) (do (do (merge l a (do b o2')) o2) o1)) 
           
 let comm_ind_right (l a b:concrete_st) (o1 o2' o2:op_t)
-  : Lemma (requires Either? (rc o1 o2) /\ Either? (rc_s (get_op_s o1) (get_op_s o2)) /\ 
+  : Lemma (requires Either? (rc o1 o2) /\ 
                     eq (merge l (do a o1) (do b o2)) (do (do (merge l a b) o2) o1))                    
           (ensures eq (merge l (do a o1) (do (do b o2') o2)) (do (do (merge l a (do b o2')) o2) o1)) =
   let k = get_key o2' in
@@ -163,19 +741,18 @@ let comm_ind_right (l a b:concrete_st) (o1 o2' o2:op_t)
   else comm_ind_right_ne l a b o1 o2' o2
 
 //simpler MRDT lemma (Already proved for Grows-only set)
-val comm_ind_left_s (l a b:concrete_st_s) (o1 o2' o2:(nat & (nat & op_s)))
-  : Lemma (requires Either? (rc_s o1 o2) /\
-                    eq_s (merge_s l (do_s a o1) (do_s b o2)) (do_s (do_s (merge_s l a b) o2) o1))
+val comm_ind_left_s (l a b:concrete_st_s) (o1 o2' o2:op_s)
+  : Lemma (requires eq_s (merge_s l (do_s a o1) (do_s b o2)) (do_s (do_s (merge_s l a b) o2) o1))
           (ensures eq_s (merge_s l (do_s (do_s a o2') o1) (do_s b o2)) (do_s (do_s (merge_s l (do_s a o2') b) o2) o1))
 
 val comm_ind_left_ne (l a b:concrete_st) (o1 o2' o2:op_t)
-  : Lemma (requires Either? (rc o1 o2) /\ Either? (rc_s (get_op_s o1) (get_op_s o2)) /\
+  : Lemma (requires Either? (rc o1 o2) /\ 
                     ~ (get_key o1 = get_key o2 /\ get_key o2 = get_key o2') /\
                     eq (merge l (do a o1) (do b o2)) (do (do (merge l a b) o2) o1))                    
           (ensures eq (merge l (do (do a o2') o1) (do b o2)) (do (do (merge l (do a o2') b) o2) o1)) 
           
 let comm_ind_left (l a b:concrete_st) (o1 o2' o2:op_t)
-  : Lemma (requires Either? (rc o1 o2) /\ Either? (rc_s (get_op_s o1) (get_op_s o2)) /\ 
+  : Lemma (requires Either? (rc o1 o2) /\ 
                     eq (merge l (do a o1) (do b o2)) (do (do (merge l a b) o2) o1))                    
           (ensures eq (merge l (do (do a o2') o1) (do b o2)) (do (do (merge l (do a o2') b) o2) o1)) =
   let k = get_key o2' in
@@ -186,19 +763,18 @@ let comm_ind_left (l a b:concrete_st) (o1 o2' o2:op_t)
   else comm_ind_left_ne l a b o1 o2' o2
 
 //simpler MRDT lemma (Already proved for Grows-only set)
-val comm_ind_lca_s (l:concrete_st_s) (ol o1 o2:(nat & (nat & op_s)))
-  : Lemma (requires Either? (rc_s o1 o2) /\
-                    eq_s (merge_s l (do_s l o1) (do_s l o2)) (do_s (do_s l o2) o1))
+val comm_ind_lca_s (l:concrete_st_s) (ol o1 o2:op_s)
+  : Lemma (requires eq_s (merge_s l (do_s l o1) (do_s l o2)) (do_s (do_s l o2) o1))
           (ensures eq_s (merge_s (do_s l ol) (do_s (do_s l ol) o1) (do_s (do_s l ol) o2)) (do_s (do_s (do_s l ol) o2) o1))
 
 val comm_ind_lca_ne (l:concrete_st) (ol o1 o2:op_t)
-  : Lemma (requires Either? (rc o1 o2) /\ Either? (rc_s (get_op_s o1) (get_op_s o2)) /\
+  : Lemma (requires Either? (rc o1 o2) /\ 
                     ~ (get_key ol = get_key o1 /\ get_key ol = get_key o2) /\
                     eq (merge l (do l o1) (do l o2)) (do (do l o2) o1))
           (ensures eq (merge (do l ol) (do (do l ol) o1) (do (do l ol) o2)) (do (do (do l ol) o2) o1)) 
           
 let comm_ind_lca (l:concrete_st) (ol o1 o2:op_t)
-  : Lemma (requires Either? (rc o1 o2) /\ Either? (rc_s (get_op_s o1) (get_op_s o2)) /\ 
+  : Lemma (requires Either? (rc o1 o2) /\
                     eq (merge l (do l o1) (do l o2)) (do (do l o2) o1))
           (ensures eq (merge (do l ol) (do (do l ol) o1) (do (do l ol) o2)) (do (do (do l ol) o2) o1)) =
   let k = get_key ol in
@@ -208,6 +784,165 @@ let comm_ind_lca (l:concrete_st) (ol o1 o2:op_t)
   else comm_ind_lca_ne l ol o1 o2
 
 val comm_base (o1 o2:op_t)
-  : Lemma (requires distinct_ops o1 o2 /\ Either? (rc o1 o2))
+  : Lemma (requires Either? (rc o1 o2) /\ distinct_ops o1 o2)
           (ensures eq (merge init_st (do init_st o1) (do init_st o2)) (do (do init_st o1) o2))
 
+val comm_inter_base_right_s (l a b c:concrete_st_s) (o1 o2 ob ol:op_s) 
+  : Lemma (requires rc_s ob ol <> Either /\ 
+                    distinct_ops o1 o2 /\ distinct_ops o1 ob /\ distinct_ops o1 ol /\ distinct_ops o2 ob /\ distinct_ops o2 ol /\ distinct_ops ob ol /\
+                    eq_s (merge_s (do_s l ol) (do_s (do_s a ol) o1) (do_s (do_s b ol) o2)) (do_s (do_s (do_s c ol) o1) o2) /\ 
+                    eq_s (merge_s l (do_s a o1) (do_s b o2)) (do_s (do_s c o1) o2) /\
+                    eq_s (merge_s l (do_s a o1) (do_s (do_s b ob) o2)) (do_s (do_s (merge_s l a (do_s b ob)) o1) o2) /\ //comes from comm_ind_right
+                    eq_s (merge_s (do_s l ol) (do_s a ol) (do_s (do_s b ob) ol)) (do_s (do_s c ob) ol)) //comes from intermediate_base_zero_op
+          (ensures eq_s (merge_s (do_s l ol) (do_s (do_s a ol) o1) (do_s (do_s (do_s b ob) ol) o2)) (do_s (do_s (do_s (do_s c ob) ol) o1) o2))
+
+val comm_inter_base_right_ne (l a b c:concrete_st) (o1 o2 ob ol:op_t) 
+  : Lemma (requires Fst_then_snd? (rc ob ol) /\ 
+                    distinct_ops o1 o2 /\ distinct_ops o1 ob /\ distinct_ops o1 ol /\ distinct_ops o2 ob /\ distinct_ops o2 ol /\ distinct_ops ob ol /\
+                    ~ (get_key o2 = get_key o1 /\ get_key o1 = get_key ob) /\
+                    eq (merge (do l ol) (do (do a ol) o1) (do (do b ol) o2)) (do (do (do c ol) o1) o2) /\ 
+                    eq (merge l (do a o1) (do b o2)) (do (do c o1) o2) /\
+                    eq (merge l (do a o1) (do (do b ob) o2)) (do (do (merge l a (do b ob)) o1) o2) /\ //comes from comm_ind_right
+                    eq (merge (do l ol) (do a ol) (do (do b ob) ol)) (do (do c ob) ol)) //comes from intermediate_base_zero_op
+          (ensures eq (merge (do l ol) (do (do a ol) o1) (do (do (do b ob) ol) o2)) (do (do (do (do c ob) ol) o1) o2)) 
+          
+let comm_inter_base_right (l a b c:concrete_st) (o1 o2 ob ol:op_t) 
+  : Lemma (requires Either? (rc o1 o2) /\ Fst_then_snd? (rc ob ol) /\ 
+                    distinct_ops o1 o2 /\ distinct_ops o1 ob /\ distinct_ops o1 ol /\ distinct_ops o2 ob /\ distinct_ops o2 ol /\ distinct_ops ob ol /\
+                    eq (merge (do l ol) (do (do a ol) o1) (do (do b ol) o2)) (do (do (do c ol) o1) o2) /\ 
+                    eq (merge l (do a o1) (do b o2)) (do (do c o1) o2) /\
+                    eq (merge l (do a o1) (do (do b ob) o2)) (do (do (merge l a (do b ob)) o1) o2) /\ //comes from comm_ind_right
+                    eq (merge (do l ol) (do a ol) (do (do b ob) ol)) (do (do c ob) ol)) //comes from intermediate_base_zero_op
+          (ensures eq (merge (do l ol) (do (do a ol) o1) (do (do (do b ob) ol) o2)) (do (do (do (do c ob) ol) o1) o2)) =
+  let k = get_key ob in
+  let l' = sel l k in let a' = sel a k in let b' = sel b k in let c' = sel c k in
+  if get_key o2 = get_key o1 && get_key o1 = k then 
+    comm_inter_base_right_s l' a' b' c' (get_op_s o1) (get_op_s o2) (get_op_s ob) (get_op_s ol)
+  else comm_inter_base_right_ne l a b c o1 o2 ob ol
+
+val comm_inter_base_left_s (l a b c:concrete_st_s) (o1 o2 ob ol:op_s) 
+  : Lemma (requires rc_s ob ol <> Either /\ 
+                    distinct_ops o1 o2 /\ distinct_ops o1 ob /\ distinct_ops o1 ol /\ distinct_ops o2 ob /\ distinct_ops o2 ol /\ distinct_ops ob ol /\
+                    eq_s (merge_s (do_s l ol) (do_s (do_s a ol) o1) (do_s (do_s b ol) o2)) (do_s (do_s (do_s c ol) o1) o2) /\ 
+                    eq_s (merge_s l (do_s a o1) (do_s b o2)) (do_s (do_s c o1) o2) /\
+                    eq_s (merge_s l (do_s (do_s a ob) o1) (do_s b o2)) (do_s (do_s (merge_s l (do_s a ob) b) o1) o2) /\ //comes from comm_ind_left
+                    eq_s (merge_s (do_s l ol) (do_s (do_s a ob) ol) (do_s b ol)) (do_s (do_s c ob) ol)) //comes from intermediate_base_zero_op
+          (ensures eq_s (merge_s (do_s l ol) (do_s (do_s (do_s a ob) ol) o1) (do_s (do_s b ol) o2)) (do_s (do_s (do_s (do_s c ob) ol) o1) o2))
+
+val comm_inter_base_left_ne (l a b c:concrete_st) (o1 o2 ob ol:op_t) 
+  : Lemma (requires Fst_then_snd? (rc ob ol) /\ 
+                    distinct_ops o1 o2 /\ distinct_ops o1 ob /\ distinct_ops o1 ol /\ distinct_ops o2 ob /\ distinct_ops o2 ol /\ distinct_ops ob ol /\
+                    ~ (get_key o2 = get_key o1 /\ get_key o1 = get_key ob) /\
+                    eq (merge (do l ol) (do (do a ol) o1) (do (do b ol) o2)) (do (do (do c ol) o1) o2) /\ 
+                    eq (merge l (do a o1) (do b o2)) (do (do c o1) o2) /\
+                    eq (merge l (do (do a ob) o1) (do b o2)) (do (do (merge l (do a ob) b) o1) o2) /\ //comes from comm_ind_left
+                    eq (merge (do l ol) (do (do a ob) ol) (do b ol)) (do (do c ob) ol)) //comes from intermediate_base_zero_op
+          (ensures eq (merge (do l ol) (do (do (do a ob) ol) o1) (do (do b ol) o2)) (do (do (do (do c ob) ol) o1) o2))
+
+let comm_inter_base_left (l a b c:concrete_st) (o1 o2 ob ol:op_t) 
+  : Lemma (requires Either? (rc o1 o2) /\ Fst_then_snd? (rc ob ol) /\ 
+                    distinct_ops o1 o2 /\ distinct_ops o1 ob /\ distinct_ops o1 ol /\ distinct_ops o2 ob /\ distinct_ops o2 ol /\ distinct_ops ob ol /\
+                    eq (merge (do l ol) (do (do a ol) o1) (do (do b ol) o2)) (do (do (do c ol) o1) o2) /\ 
+                    eq (merge l (do a o1) (do b o2)) (do (do c o1) o2) /\
+                    eq (merge l (do (do a ob) o1) (do b o2)) (do (do (merge l (do a ob) b) o1) o2) /\ //comes from comm_ind_left
+                    eq (merge (do l ol) (do (do a ob) ol) (do b ol)) (do (do c ob) ol)) //comes from intermediate_base_zero_op
+          (ensures eq (merge (do l ol) (do (do (do a ob) ol) o1) (do (do b ol) o2)) (do (do (do (do c ob) ol) o1) o2)) =
+  let k = get_key ob in
+  let l' = sel l k in let a' = sel a k in let b' = sel b k in let c' = sel c k in
+  if get_key o2 = get_key o1 && get_key o1 = k then 
+    comm_inter_base_left_s l' a' b' c' (get_op_s o1) (get_op_s o2) (get_op_s ob) (get_op_s ol)
+  else comm_inter_base_left_ne l a b c o1 o2 ob ol
+
+val comm_inter_right_s (l a b c:concrete_st_s) (o1 o2 ob ol o:op_s)
+  : Lemma (requires rc_s ob ol <> Either /\ 
+                    distinct_ops o1 o2 /\ distinct_ops o1 ob /\ distinct_ops o1 ol /\ distinct_ops o1 o /\ distinct_ops o2 ob /\ 
+                    distinct_ops o2 ol /\ distinct_ops o2 o /\ distinct_ops ob ol /\ distinct_ops ob o /\ distinct_ops ol o /\
+                    get_rid o <> get_rid ol (*o,ol must be concurrent*) /\
+                    eq_s (merge_s (do_s l ol) (do_s (do_s a ol) o1) (do_s (do_s (do_s b ob) ol) o2)) (do_s (do_s (do_s (do_s c ob) ol) o1) o2))
+          (ensures eq_s (merge_s (do_s l ol) (do_s (do_s a ol) o1) (do_s (do_s (do_s (do_s b o) ob) ol) o2)) (do_s (do_s (do_s (do_s (do_s c o) ob) ol) o1) o2))
+          
+val comm_inter_right_ne (l a b c:concrete_st) (o1 o2 ob ol o:op_t)
+  : Lemma (requires Either? (rc o1 o2) /\ Fst_then_snd? (rc ob ol) /\ 
+                    distinct_ops o1 o2 /\ distinct_ops o1 ob /\ distinct_ops o1 ol /\ distinct_ops o1 o /\ distinct_ops o2 ob /\ 
+                    distinct_ops o2 ol /\ distinct_ops o2 o /\ distinct_ops ob ol /\ distinct_ops ob o /\ distinct_ops ol o /\
+                    ~ (get_key o1 = get_key o2 /\ get_key o2 = get_key ob) /\
+                    get_rid o <> get_rid ol (*o,ol must be concurrent*) /\
+                    //Either? (rc o ol) /\ 
+                    ((~ (commutes_with o ob)) \/ Fst_then_snd? (rc o ol)) /\
+                    eq (merge (do l ol) (do (do a ol) o1) (do (do (do b ob) ol) o2)) (do (do (do (do c ob) ol) o1) o2))
+          (ensures eq (merge (do l ol) (do (do a ol) o1) (do (do (do (do b o) ob) ol) o2)) (do (do (do (do (do c o) ob) ol) o1) o2))
+  
+let comm_inter_right (l a b c:concrete_st) (o1 o2 ob ol o:op_t)
+  : Lemma (requires Either? (rc o1 o2) /\ Fst_then_snd? (rc ob ol) /\ 
+                    distinct_ops o1 o2 /\ distinct_ops o1 ob /\ distinct_ops o1 ol /\ distinct_ops o1 o /\ distinct_ops o2 ob /\ 
+                    distinct_ops o2 ol /\ distinct_ops o2 o /\ distinct_ops ob ol /\ distinct_ops ob o /\ distinct_ops ol o /\
+                    get_rid o <> get_rid ol (*o,ol must be concurrent*) /\
+                    //Either? (rc o ol) /\ 
+                    ((~ (commutes_with o ob)) \/ Fst_then_snd? (rc o ol)) /\
+                    eq (merge (do l ol) (do (do a ol) o1) (do (do (do b ob) ol) o2)) (do (do (do (do c ob) ol) o1) o2))
+          (ensures eq (merge (do l ol) (do (do a ol) o1) (do (do (do (do b o) ob) ol) o2)) (do (do (do (do (do c o) ob) ol) o1) o2)) =
+    let k = get_key o in
+  let l' = sel l k in let a' = sel a k in let b' = sel b k in let c' = sel c k in
+  if get_key o2 = get_key o1 && get_key o1 = k then 
+    comm_inter_right_s l' a' b' c' (get_op_s o1) (get_op_s o2) (get_op_s ob) (get_op_s ol) (get_op_s o)
+  else comm_inter_right_ne l a b c o1 o2 ob ol o
+
+val comm_inter_left_s (l a b c:concrete_st_s) (o1 o2 ob ol o:op_s)
+  : Lemma (requires rc_s ob ol <> Either /\ 
+                    distinct_ops o1 o2 /\ distinct_ops o1 ob /\ distinct_ops o1 ol /\ distinct_ops o1 o /\ distinct_ops o2 ob /\ 
+                    distinct_ops o2 ol /\ distinct_ops o2 o /\ distinct_ops ob ol /\ distinct_ops ob o /\ distinct_ops ol o /\
+                    get_rid o <> get_rid ol (*o,ol must be concurrent*) /\
+                    eq_s (merge_s (do_s l ol) (do_s (do_s (do_s a ob) ol) o1) (do_s (do_s b ol) o2)) (do_s (do_s (do_s (do_s c ob) ol) o1) o2))
+          (ensures eq_s (merge_s (do_s l ol) (do_s (do_s (do_s (do_s a o) ob) ol) o1) (do_s (do_s b ol) o2)) (do_s (do_s (do_s (do_s (do_s c o) ob) ol) o1) o2))
+          
+val comm_inter_left_ne (l a b c:concrete_st) (o1 o2 ob ol o:op_t)
+  : Lemma (requires Either? (rc o1 o2) /\ Fst_then_snd? (rc ob ol) /\ 
+                    distinct_ops o1 o2 /\ distinct_ops o1 ob /\ distinct_ops o1 ol /\ distinct_ops o1 o /\ distinct_ops o2 ob /\ 
+                    distinct_ops o2 ol /\ distinct_ops o2 o /\ distinct_ops ob ol /\ distinct_ops ob o /\ distinct_ops ol o /\
+                    ~ (get_key o1 = get_key o2 /\ get_key o2 = get_key ob) /\
+                    get_rid o <> get_rid ol (*o,ol must be concurrent*) /\
+                    //Either? (rc o ol) /\ 
+                    ((~ (commutes_with o ob)) \/ Fst_then_snd? (rc o ol)) /\
+                    eq (merge (do l ol) (do (do (do a ob) ol) o1) (do (do b ol) o2)) (do (do (do (do c ob) ol) o1) o2))
+          (ensures eq (merge (do l ol) (do (do (do (do a o) ob) ol) o1) (do (do b ol) o2)) (do (do (do (do (do c o) ob) ol) o1) o2))
+  
+let comm_inter_left (l a b c:concrete_st) (o1 o2 ob ol o:op_t)
+  : Lemma (requires Either? (rc o1 o2) /\ Fst_then_snd? (rc ob ol) /\ 
+                    distinct_ops o1 o2 /\ distinct_ops o1 ob /\ distinct_ops o1 ol /\ distinct_ops o1 o /\ distinct_ops o2 ob /\ 
+                    distinct_ops o2 ol /\ distinct_ops o2 o /\ distinct_ops ob ol /\ distinct_ops ob o /\ distinct_ops ol o /\
+                    get_rid o <> get_rid ol (*o,ol must be concurrent*) /\
+                    //Either? (rc o ol) /\ 
+                    ((~ (commutes_with o ob)) \/ Fst_then_snd? (rc o ol)) /\
+                    eq (merge (do l ol) (do (do (do a ob) ol) o1) (do (do b ol) o2)) (do (do (do (do c ob) ol) o1) o2))
+          (ensures eq (merge (do l ol) (do (do (do (do a o) ob) ol) o1) (do (do b ol) o2)) (do (do (do (do (do c o) ob) ol) o1) o2)) =
+    let k = get_key o in
+  let l' = sel l k in let a' = sel a k in let b' = sel b k in let c' = sel c k in
+  if get_key o2 = get_key o1 && get_key o1 = k then 
+    comm_inter_left_s l' a' b' c' (get_op_s o1) (get_op_s o2) (get_op_s ob) (get_op_s ol) (get_op_s o)
+  else comm_inter_left_ne l a b c o1 o2 ob ol o
+
+val comm_inter_lca_s (l a b c:concrete_st_s) (o1 o2 ol:op_s)
+  : Lemma (requires distinct_ops o1 o2 /\ distinct_ops o1 ol /\ distinct_ops ol o2 /\
+                    (exists o'. rc_s o' ol <> Either) /\
+                    eq_s (merge_s l (do_s a o1) (do_s b o2)) (do_s (do_s c o1) o2))
+          (ensures eq_s (merge_s (do_s l ol) (do_s (do_s a ol) o1) (do_s (do_s b ol) o2)) (do_s (do_s (do_s c ol) o1) o2))
+
+val comm_inter_lca_ne (l a b c:concrete_st) (o1 o2 ol:op_t)
+  : Lemma (requires Either? (rc o1 o2) /\ 
+                    distinct_ops o1 o2 /\ distinct_ops o1 ol /\ distinct_ops ol o2 /\
+                    ~ ( get_key o2 = get_key o1 /\ get_key o1 = get_key ol) /\
+                    (exists o'. Fst_then_snd? (rc o' ol)) /\
+                    eq (merge l (do a o1) (do b o2)) (do (do c o1) o2))
+          (ensures eq (merge (do l ol) (do (do a ol) o1) (do (do b ol) o2)) (do (do (do c ol) o1) o2)) 
+          
+let comm_inter_lca (l a b c:concrete_st) (o1 o2 ol:op_t)
+  : Lemma (requires Either? (rc o1 o2) /\ 
+                    distinct_ops o1 o2 /\ distinct_ops o1 ol /\ distinct_ops ol o2 /\
+                    (exists o'. Fst_then_snd? (rc o' ol)) /\
+                    eq (merge l (do a o1) (do b o2)) (do (do c o1) o2))
+          (ensures eq (merge (do l ol) (do (do a ol) o1) (do (do b ol) o2)) (do (do (do c ol) o1) o2)) =
+  let k = get_key ol in
+  let l' = sel l k in let a' = sel a k in let b' = sel b k in let c' = sel c k in
+  if get_key o2 = get_key o1 && get_key o1 = k then 
+    comm_inter_lca_s l' a' b' c' (get_op_s o1) (get_op_s o2) (get_op_s ol)
+  else comm_inter_lca_ne l a b c o1 o2 ol
